theories/stacked_borrows/examples/opt1_down.v
@@ -44,13 +44,15 @@ Definition ex1_down_opt : ectx :=
     "v"
   .
 
+(*Lemma value_rel_poison *)
+
 Lemma sim_opt1_down `{sborG Σ} π :
   ⊢ sim_ectx rrel π ex1_down_opt ex1_down_unopt rrel.
 Proof.
   iIntros (r_t r_s) "Hrel".
   sim_pures.
   sim_apply InitCall InitCall sim_init_call "". iIntros (c) "Hcall". iApply sim_expr_base. sim_pures.
-  sim_apply (Alloc _) (Alloc _) sim_alloc_local "". iIntros (t l_t l_s) "Htag Ht Hs".
+  sim_apply (Alloc _) (Alloc _) sim_alloc_local "". iIntros (t l) "Htag Ht Hs".
   iApply sim_expr_base. sim_pures. simpl.
 
   source_bind (Write _ _).
@@ -74,8 +76,8 @@ Proof.
   iIntros ((_ & ot & i & -> & _)).
   iPoseProof (value_rel_singleton_source with "Hv") as (sc_t) "[-> Hscrel]".
   iPoseProof (sc_rel_ptr_source with "Hscrel") as "[-> Htagged]". 
-  iApply (sim_retag_fnentry with "Hscrel Hcall"); [cbn; lia| ].
-  iIntros (t_i v_t v_s Hlen_t Hlen_s) "Hvrel Hcall Htag_i Hi_t Hi_s _".
+  iApply (sim_retag_fnentry with "Hscrel Hcall"); [cbn; lia| done | ].
+  iIntros (t_i v_t v_s Hlen_t Hlen_s) "#Hvrel Hcall Htag_i Hi_t Hi_s _".
   iApply sim_expr_base.
   target_apply (Write _ _) (target_write_local with "Htag Ht") "Ht Htag"; [done | done | ].
   source_apply (Write _ _) (source_write_local with "Htag Hs") "Hs Htag"; [done | done | ].
@@ -83,7 +85,8 @@ Proof.
 
   (* do the source load *)
   source_apply (Copy (Place _ _ _)) (source_copy_local with "Htag Hs") "Hs Htag"; first done.
-  source_pures. source_apply (Copy _) (source_copy_any with "Htag_i Hi_s") "Hi_s Htag_i"; first done. 
+  source_pures. source_bind (Copy _).  
+  iApply (source_copy_any with "Htag_i Hi_s"); first done. iIntros (v_s' Hv_s') "Hi_s Htag_i". source_finish.
   sim_pures.
 
   sim_apply (Call _ _) (Call _ _) (sim_call _ _ (ValR []) (ValR [])) ""; first by iApply value_rel_empty.
@@ -95,8 +98,28 @@ Proof.
   { simpl. intros i0 Hi0. assert (i0 = O) as -> by lia. eexists. split; first apply lookup_insert.  set_solver. } 
   sim_pures. 
 
-  sim_bind (Free _) (Free _).
-  (* TODO: need local free lemma that also removes the ghost state for that *)
+  (* cleanup: remove the protector ghost state, make the external locations public, free the local locations*)
+  sim_apply (Free _) (Free _) (sim_free_local with "Htag Ht Hs") "". sim_pures.
+  iApply (sim_protected_unprotectN with "Hcall Htag_i Hi_t Hi_s Hvrel"); [ | apply lookup_insert | ].
+  { simpl. cbn in Hlen_t. intros i' Hi'. replace i' with O by lia. rewrite elem_of_union elem_of_singleton. eauto. } 
+  iIntros "Hcall Htag_i Hi_t Hi_s".
+  iApply (sim_remove_empty_calls _ t_i with "Hcall"). 
+  { rewrite lookup_insert. done. } 
+  { rewrite Hlen_t. set_solver. } 
+  iIntros "Hcall".
+  sim_apply (EndCall _) (EndCall _) (sim_endcall with "[Hcall]") "".
+  { replace (delete t_i _) with (∅ : gmap ptr_id (gset loc)); first done. 
+    apply map_eq. intros t'. rewrite delete_insert_delete delete_insert; done.
+  } 
+  sim_pures. 
+  sim_val. iModIntro. destruct Hv_s' as [-> | ->]; first done. 
+  iApply big_sepL2_forall. iSplit. { rewrite replicate_length. iPureIntro. lia. } 
+  iIntros (k sc_t sc_s). rewrite lookup_replicate. iIntros "Hsc (-> & _)". 
+  (* TODO: fix the pointer refined by poison thing in the relation *)
+  (*destruct sc_t; done.*)
+  
+  (*iApply big_sepL2_singleton; done.*)
+
 Abort.
 
 
