theories/stacked_borrows/steps_opt.v
@@ -1,0 +1,862 @@
+From iris.proofmode Require Export tactics.
+From iris.bi.lib Require Import fractional.
+From iris.base_logic.lib Require Import ghost_map.
+From simuliris.base_logic Require Export gen_sim_prog.
+From simuliris.simulation Require Export slsls.
+From simuliris.simulation Require Import lifting.
+From iris.prelude Require Import options.
+From simuliris.stacked_borrows Require Import tkmap_view.
+From simuliris.stacked_borrows Require Export defs.
+From simuliris.stacked_borrows Require Import steps_progress steps_retag steps_inv.
+From simuliris.stacked_borrows Require Import heap.
+
+Section lifting.
+Context `{!sborG Σ}.
+Implicit Types P Q : iProp Σ.
+Implicit Types Φ : expr → expr → iProp Σ.
+Implicit Types σ σ_s σ_t : state.
+Implicit Types r r_s r_t : result.
+Implicit Types l : loc.
+Implicit Types f : fname.
+
+Context (Ω : result → result → iProp Σ).
+
+
+(** Retags *)
+Lemma bor_interp_retag_default σ_t σ_s c l ot T α' mut :
+  let pk : pointer_kind := RefPtr mut in
+  let pm := match mut with Mutable => Unique | Immutable => SharedReadOnly end in
+  let tk := match mut with Mutable => tk_unq | Immutable => tk_pub end in
+  retag σ_s.(sst) σ_s.(snp) σ_s.(scs) c l ot Default pk T = Some (Tagged σ_s.(snp), α', S σ_s.(snp)) →
+  c ∈ σ_s.(scs) →
+  (if mut is Immutable then is_freeze T else True) →
+  state_wf (mkState σ_t.(shp) α' σ_t.(scs) (S σ_t.(snp)) σ_t.(snc)) →   (* could remove that assumption *)
+  state_wf (mkState σ_s.(shp) α' σ_s.(scs) (S σ_s.(snp)) σ_s.(snc)) →   (* could remove that assumption *)
+  sc_rel (ScPtr l ot) (ScPtr l ot) -∗
+  bor_interp sc_rel σ_t σ_s ==∗ ∃ v_t v_s,
+  ⌜length v_t = tsize T⌝ ∗
+  ⌜length v_s = tsize T⌝ ∗
+  value_rel v_t v_s ∗
+  σ_t.(snp) $$ tk ∗
+  l ↦t∗[tk]{σ_t.(snp)} v_t ∗
+  l ↦s∗[tk]{σ_t.(snp)} v_s ∗
+  match mut with
+  | Mutable => True
+  | Immutable =>
+    sc_rel (ScPtr l (Tagged (σ_t.(snp)))) (ScPtr l (Tagged (σ_t.(snp))))
+  end ∗
+  bor_interp sc_rel (mkState σ_t.(shp) α' σ_t.(scs) (S σ_t.(snp)) σ_t.(snc)) (mkState σ_s.(shp) α' σ_s.(scs) (S σ_s.(snp)) σ_s.(snc)).
+Proof.
+  intros pk pm tk Hretag Hc_in Hfreeze Hwf'_t Hwf'_s.
+  iIntros "Hscrel Hbor". iDestruct "Hbor" as "(% & % & % & % & (Hc & Htag_auth & Htag_t_auth & Htag_s_auth) & #Hsrel & %Hcall_interp & %Htag_interp & %Hwf_s & %Hwf_t)".
+
+  iDestruct "Hscrel" as "[_ Hrel]".
+  iAssert (⌜untagged_or_public M_tag ot⌝)%I as %Hpub.
+  { iDestruct "Hrel" as "[[-> _] | (%t1 & %t2 & -> & -> & <- & Hpub)]"; first done.
+    iPoseProof (tkmap_lookup with "Htag_auth Hpub") as "%". done.
+  }
+  pose nt := (snp σ_t).
+
+  have Hin_dom := retag_Some_dom _ _ _ _ _ _ _ pk _ _ _ _ I Hretag.
+  iPoseProof (state_rel_dom_eq with "Hsrel") as "%Hdom_eq".
+  destruct (read_mem_is_Some l (tsize T) σ_s.(shp)) as [v_s Hv_s].
+  { setoid_rewrite (state_wf_dom _ Hwf_s). done. }
+  destruct (read_mem_is_Some l (tsize T) σ_t.(shp)) as [v_t Hv_t].
+  { rewrite Hdom_eq. setoid_rewrite (state_wf_dom _ Hwf_s). done. }
+  destruct (read_mem_values _ _ _ _ Hv_s) as [Hlen_s Hshp_s].
+  destruct (read_mem_values _ _ _ _ Hv_t) as [Hlen_t Hshp_t].
+
+  (* allocate resources *)
+  assert (M_tag !! nt = None) as Htag_none.
+  { destruct (M_tag !! nt) as [[tk' []] | ] eqn:Ht_some; last done.
+    apply Htag_interp in Ht_some as [Hcontra _]. lia. }
+  destruct Htag_interp as (Htag_interp & Ht_dom & Hs_dom).
+  iMod (tkmap_insert tk _ tt Htag_none with "Htag_auth") as "[Htag_auth Hnt]".
+  iMod (ghost_map_array_tag_insert _ _ v_t nt l with "Htag_t_auth") as "[Ht Htag_t_auth]".
+  { intros i Hi. destruct (M_t !! (nt, l +ₗ i)) eqn:Hmt; last done.
+    destruct (Ht_dom nt (l +ₗ i) ltac:(eauto)) as (? & ?); congruence. }
+  iMod (ghost_map_array_tag_insert _ _ v_s nt l with "Htag_s_auth") as "[Hs Htag_s_auth]".
+  { intros i Hi. destruct (M_s !! (nt, l +ₗ i)) eqn:Hmt; last done.
+    destruct (Hs_dom nt (l +ₗ i) ltac:(eauto)) as (? & ?); congruence. }
+  iMod (ghost_map_array_tag_tk _ _ _ _ tk with "Ht") as "Ht".
+  iMod (ghost_map_array_tag_tk _ _ _ _ tk with "Hs") as "Hs".
+  iModIntro.
+  iAssert (nt $$ tk ∗ if tk is tk_pub then nt $$ tk_pub else True)%I  with "[Hnt]" as "[$ Hpubt]".
+  { destruct tk; eauto. }
+  iExists v_t, v_s. iSplit; first done. iSplit; first done. iFrame "Ht Hs".
+
+  iAssert (⌜retag σ_t.(sst) σ_t.(snp) σ_t.(scs) c l ot Default pk T = Some (Tagged nt, α', S (σ_t.(snp)))⌝)%I as "%Hretag_t".
+  { iPoseProof (state_rel_calls_eq with "Hsrel") as "<-".
+    iPoseProof (state_rel_stacks_eq with "Hsrel") as "<-".
+    subst nt. iPoseProof (state_rel_snp_eq with "Hsrel") as "<-". done. }
+  (* proving the value relation *)
+  iAssert (value_rel v_t v_s)%I as "#Hvrel"; last iFrame "Hvrel".
+  { iApply big_sepL2_forall; iSplit; first (iPureIntro;lia).
+    iIntros (i sc_t sc_s) "%Hs_t %Hs_v".
+    assert (i < tsize T)%nat as Hi. { rewrite -Hlen_t. eapply lookup_lt_is_Some_1. eauto. }
+    assert (Hsome_target : is_Some (σ_t.(shp) !! (l +ₗ i))).
+    { rewrite Hshp_t; last done. apply lookup_lt_is_Some_2. by rewrite Hlen_t. }
+    iPoseProof (state_rel_pub_if_not_priv _ _ _ _ _ _ (l +ₗ i) with "[] Hsrel [Hrel]") as "Hpub"; first done.
+    { iPoseProof (state_rel_calls_eq with "Hsrel") as "%Hcall_eq".
+      iPoseProof (state_rel_stacks_eq with "Hsrel") as "%Hstack_eq".
+      iPureIntro. intros t Hpriv.
+      eapply (priv_loc_UB_retag_access_eq σ_s σ_t); eauto; done. }
+    iPoseProof (pub_loc_lookup with "[] Hpub") as "(%sc_t' & %sc_s' & %Hread_both & Hsc_rel)"; first done.
+    enough (sc_t = sc_t' ∧ sc_s = sc_s') by naive_solver.
+    move : Hs_t Hs_v Hread_both (Hshp_s i Hi) (Hshp_t i Hi).
+    by move => -> -> [-> ->] [= ->] [= ->].
+  }
+
+  iSplitL "Hpubt".
+  { destruct mut; first done. iSplitR; first done. iRight.
+    iExists (σ_t.(snp)), (σ_t.(snp)). do 3 (iSplitR; first done). done. }
+
+  (* re-establishing the interpretation *)
+  iExists M_call, (<[ nt := (tk, ()) ]> M_tag), (array_tag_map l nt v_t ∪ M_t), (array_tag_map l nt v_s ∪ M_s).
+  iFrame. iSplitL.
+  { (* state relation *)
+    rewrite /state_rel. simpl. iDestruct "Hsrel" as "(-> & %Hs_eq & -> & -> & -> & Hsrel)".
+    do 5 (iSplitL; first done). iIntros (l' Hsl').
+    iDestruct ("Hsrel" $! l' with "[//]") as "[Hpub | [%t' %Hpriv]]"; first (iLeft; iApply "Hpub").
+    iRight. iPureIntro. exists t'.
+    destruct Hpriv as (tk' & Hsome_tk' & Ht_l' & Htk'). exists tk'.
+    assert (t' ≠ nt). { intros ->. simplify_eq. }
+    rewrite lookup_insert_ne; last done.
+    split; first done. split; last done.
+    destruct Ht_l' as (sc0 & Ht_l'). exists sc0.
+    rewrite lookup_union_r; first done.
+    destruct (array_tag_map l nt v_t !! (t', l')) as [ a | ] eqn:Harr; last done.
+    specialize (array_tag_map_lookup1 l nt v_t t' l' ltac:(eauto)) as [Heq _]. congruence.
+  }
+  iSplitL.
+  { (* call interpretation. *)
+    iPureIntro. intros c' M' [Hc' HM']%Hcall_interp. split; first done.
+    intros t' S HS. simpl. specialize (HM' t' S HS) as (Ht' & Hprot).
+    split; first lia. intros l' Hl'.
+    specialize (Hprot l' Hl') as (s & pm' & Hs & Hit & Hpm').
+    specialize (retag_item_active_preserving _ _ _ _ _ _ _ _ _ _ _ _ Hretag_t l' s (Tagged t') c' pm' Hs Hc' Hit) as (s' & -> & Hin'). eauto.
+  }
+  iSplitL.
+  { (* tag interpretation. *)
+    iPoseProof (state_rel_get_pure with "Hsrel") as "%Hp".
+    destruct Hp as (Hsst & Hsnp & Hsnc & Hscs).
+    assert (∀l', M_t !! (nt, l') = None) as HMt_nt.
+    { intros l'. destruct (M_t !! (nt, l')) eqn:HM_t; last done.
+      specialize (Ht_dom nt l' ltac:(eauto)) as (? & ?); congruence. }
+    assert (∀l', M_s !! (nt, l') = None) as HMs_nt.
+    { intros l'. destruct (M_s !! (nt, l')) eqn:HM_s; last done.
+      specialize (Hs_dom nt l' ltac:(eauto)) as (? & ?); congruence. }
+    iPureIntro. split_and!.
+    { intros t tk'. rewrite lookup_insert_Some. intros [[<- [= <-]] | [Hneq Hsome_t]].
+      - cbn. split_and!; [lia | lia | | |].
+        + intros l' sc_t Ha%lookup_union_Some_l'; last done.
+          specialize (array_tag_map_lookup2 l nt v_t nt l' ltac:(eauto)) as [_ (i & Hi & ->)].
+          eapply retag_mut_loc_controlled; [ done | done |  done | lia | ].
+          move : Ha. rewrite array_tag_map_lookup_Some; last done. move => <-. apply Hshp_t. lia.
+        + intros l' sc_s Ha%lookup_union_Some_l'; last done.
+          specialize (array_tag_map_lookup2 l nt v_s nt l' ltac:(eauto)) as [_ (i & Hi & ->)].
+          subst nt. rewrite -Hsnp. eapply retag_mut_loc_controlled; [ done | done | done | lia | ].
+          move : Ha. rewrite array_tag_map_lookup_Some; last done. move => <-. apply Hshp_s. lia.
+        + apply dom_agree_on_tag_union. { apply dom_agree_on_tag_array_tag_map. lia. }
+          apply dom_agree_on_tag_not_elem; done.
+      - cbn.
+        specialize (Htag_interp t tk' Hsome_t) as (Ht_t & Ht_s & Hcontrolled_t & Hcontrolled_s & Hagree).
+        split_and!; [ lia | lia | | | ].
+        + intros l' sc_t Ha. rewrite lookup_union_r in Ha; last by apply array_tag_map_lookup_None.
+          apply Hcontrolled_t in Ha.
+          eapply retag_loc_controlled_preserved; [done | done | | done | done].
+          intros <-. destruct tk'; [ done | | ]; move : Hsome_t Hpub; congruence.
+        + intros l' sc_s Ha. rewrite lookup_union_r in Ha; last by apply array_tag_map_lookup_None.
+          apply Hcontrolled_s in Ha.
+          eapply retag_loc_controlled_preserved; [done | done | | done | done].
+          intros <-. destruct tk'; [ done | | ]; move : Hsome_t Hpub; congruence.
+        + apply dom_agree_on_tag_union; last done.
+          apply dom_agree_on_tag_not_elem; apply array_tag_map_lookup_None; done.
+    }
+    { intros t l'.
+      rewrite lookup_union_is_Some lookup_insert_is_Some'. intros [[-> _]%array_tag_map_lookup2 | H%Ht_dom]; eauto. }
+    { intros t l'.
+      rewrite lookup_union_is_Some lookup_insert_is_Some'. intros [[-> _]%array_tag_map_lookup2 | H%Hs_dom]; eauto. }
+  }
+  done.
+Qed.
+
+(* TODO: for Mutable, this is currently not particularly useful, since reads are UB when the tag is not there.
+  Instead, need a mechanism for "deferred observations" or such
+*)
+Lemma sim_retag_default mut T l_t l_s c ot π Φ :
+  (0 < tsize T)%nat → (* for convenience: makes the proof easier *)
+  let pk : pointer_kind := RefPtr mut in
+  let pm := match mut with Mutable => Unique | Immutable => SharedReadOnly end in
+  let tk := match mut with Mutable => tk_unq | Immutable => tk_pub end in
+  (if mut is Immutable then is_freeze T else True) →
+  sc_rel (ScPtr l_t ot) (ScPtr l_s ot) -∗
+  (∀ nt v_t v_s,
+    ⌜length v_t = tsize T⌝ -∗ ⌜length v_s = tsize T⌝ -∗
+    value_rel v_t v_s -∗  (* as the pointers were public before *)
+    nt $$ tk -∗
+    l_t ↦t∗[tk]{nt} v_t -∗
+    l_s ↦s∗[tk]{nt} v_s -∗
+    (if mut is Immutable then sc_rel (ScPtr l_t (Tagged nt)) (ScPtr l_s (Tagged nt)) else True) -∗
+    #[ScPtr l_t (Tagged nt)] ⪯{π, Ω} #[ScPtr l_s (Tagged nt)] [{ Φ }]) -∗
+  Retag #[ScPtr l_t ot] #[ScCallId c] pk T Default ⪯{π, Ω} Retag #[ScPtr l_s ot] #[ScCallId c] pk T Default [{ Φ }].
+Proof.
+  intros Hsize pk pm tk Hmut. iIntros "#Hscrel Hsim".
+  iApply sim_lift_head_step_both. iIntros (??????) "((HP_t & HP_s & Hbor) & %Hthread & %Hsafe)".
+  (* exploit source to gain knowledge about stacks & that c is a valid id *)
+  specialize (pool_safe_irred _ _ _ _ _ _ _ Hsafe Hthread ltac:(done)) as (c' & ot' & l' & [= <- <-] & [= <-] & Hc_active & Hretag_some_s).
+  iPoseProof "Hscrel" as "(-> & _)".
+  iPoseProof (bor_interp_get_pure with "Hbor") as "%Hp".
+  have Hretag_some_t : is_Some (retag σ_t.(sst) σ_t.(snp) σ_t.(scs) c l_s ot Default pk T).
+  { destruct Hp as (<- & <- & _ & <- & _). done. }
+  iModIntro. iSplitR.
+  { iPureIntro.
+    destruct Hretag_some_t as ([[] ] & Hretag_some_t).
+    do 3 eexists. eapply retag_head_step'; last done.
+    destruct Hp as (_ & _ & _ & <- & _). done.
+  }
+  iIntros (e_t' efs_t σ_t') "%Hhead_t".
+  specialize (head_retag_inv _ _ _ _ _ _ _ _ _ _ _ Hhead_t) as (nt & α' & nxtp' & Hretag_t & -> & -> & -> & Hc).
+  have Hretag_s : retag σ_s.(sst) σ_s.(snp) σ_s.(scs) c l_s ot Default pk T = Some (nt, α', nxtp').
+  { destruct Hp as (-> & -> & _ & -> & _). done. }
+  assert (Hhead_s : head_step P_s (Retag #[ScPtr l_s ot] #[ScCallId c] pk T Default) σ_s #[ScPtr l_s nt]%E (mkState (shp σ_s) α' (scs σ_s) nxtp' (snc σ_s)) []).
+  { eapply retag_head_step'; done. }
+  specialize (retag_change_ref_NZST _ _ _ _ _ _ _ _ _ _ _ _ Hsize Hretag_s) as [-> ->].
+
+  iPoseProof (bor_interp_get_state_wf with "Hbor") as "[%Hwf_t %Hwf_s]".
+  iMod (bor_interp_retag_default _ _ _ _ _ _ _ _ Hretag_s ltac:(done) with "Hscrel Hbor") as
+    (v_t v_s) "(%Hlen_t & %Hlen_s & Hval & Htag & Ht & Hs & Hpub & Hbor)"; first done.
+  { destruct Hp as (_ & <- & _). eapply head_step_wf; eauto. }
+  { eapply head_step_wf; eauto. }
+  iModIntro.
+
+  iExists #[ScPtr l_s (Tagged σ_s.(snp))]%E, [], (mkState σ_s.(shp) α' σ_s.(scs) (S σ_s.(snp)) σ_s.(snc)).
+  iSplitR; first done.
+  destruct Hp as (_ & -> & _).
+  iFrame "Hbor HP_t HP_s".
+  iSplitL; last done.
+  iApply ("Hsim" with "[] [] Hval Htag Ht Hs Hpub"); [done | done | ..].
+Qed.
+
+
+Lemma bor_interp_retag_fnentry σ_t σ_s l ot c T α' M mut :
+  let pk : pointer_kind := RefPtr mut in
+  let pm := match mut with Mutable => Unique | Immutable => SharedReadOnly end in
+  let tk := match mut with Mutable => tk_unq | Immutable => tk_pub end in
+  let L := seq_loc_set l (tsize T) in   (* uses that l_t = l_s *)
+  retag σ_s.(sst) σ_s.(snp) σ_s.(scs) c l ot FnEntry pk T = Some (Tagged σ_s.(snp), α', S σ_s.(snp)) →
+  (if mut is Immutable then is_freeze T else True) →
+  state_wf (mkState σ_t.(shp) α' σ_t.(scs) (S σ_t.(snp)) σ_t.(snc)) →   (* could remove that assumption *)
+  state_wf (mkState σ_s.(shp) α' σ_s.(scs) (S σ_s.(snp)) σ_s.(snc)) →   (* could remove that assumption *)
+  sc_rel (ScPtr l ot) (ScPtr l ot) -∗
+  c @@ M -∗
+  bor_interp sc_rel σ_t σ_s ==∗ ∃ v_t v_s,
+  ⌜length v_t = tsize T⌝ ∗
+  ⌜length v_s = tsize T⌝ ∗
+  value_rel v_t v_s ∗
+  c @@ <[σ_t.(snp) := L]> M ∗
+  σ_t.(snp) $$ tk ∗
+  l ↦t∗[tk]{σ_t.(snp)} v_t ∗
+  l ↦s∗[tk]{σ_t.(snp)} v_s ∗
+  match mut with
+  | Mutable => True
+  | Immutable =>
+    sc_rel (ScPtr l (Tagged (σ_t.(snp)))) (ScPtr l (Tagged (σ_t.(snp))))
+  end ∗
+  bor_interp sc_rel (mkState σ_t.(shp) α' σ_t.(scs) (S σ_t.(snp)) σ_t.(snc)) (mkState σ_s.(shp) α' σ_s.(scs) (S σ_s.(snp)) σ_s.(snc)).
+Proof.
+  intros pk pm tk L Hretag Hfreeze Hwf'_t Hwf'_s.
+  iIntros "Hscrel Hcid Hbor". iDestruct "Hbor" as "(% & % & % & % & (Hc & Htag_auth & Htag_t_auth & Htag_s_auth) & #Hsrel & %Hcall_interp & %Htag_interp & %Hwf_s & %Hwf_t)".
+
+  iDestruct "Hscrel" as "[_ Hrel]".
+  iAssert (⌜untagged_or_public M_tag ot⌝)%I as %Hpub.
+  { iDestruct "Hrel" as "[[-> _] | (%t1 & %t2 & -> & -> & <- & Hpub)]"; first done.
+    iPoseProof (tkmap_lookup with "Htag_auth Hpub") as "%". done.
+  }
+  pose nt := (snp σ_t).
+
+  have Hin_dom := retag_Some_dom _ _ _ _ _ _ _ pk _ _ _ _ I Hretag.
+  iPoseProof (state_rel_dom_eq with "Hsrel") as "%Hdom_eq".
+  destruct (read_mem_is_Some l (tsize T) σ_s.(shp)) as [v_s Hv_s].
+  { setoid_rewrite (state_wf_dom _ Hwf_s). done. }
+  destruct (read_mem_is_Some l (tsize T) σ_t.(shp)) as [v_t Hv_t].
+  { rewrite Hdom_eq. setoid_rewrite (state_wf_dom _ Hwf_s). done. }
+  destruct (read_mem_values _ _ _ _ Hv_s) as [Hlen_s Hshp_s].
+  destruct (read_mem_values _ _ _ _ Hv_t) as [Hlen_t Hshp_t].
+
+  (* allocate resources *)
+  assert (M_tag !! nt = None) as Htag_none.
+  { destruct (M_tag !! nt) as [[tk' []] | ] eqn:Ht_some; last done.
+    apply Htag_interp in Ht_some as [Hcontra _]. lia. }
+  destruct Htag_interp as (Htag_interp & Ht_dom & Hs_dom).
+  iMod (tkmap_insert tk _ tt Htag_none with "Htag_auth") as "[Htag_auth Hnt]".
+  iMod (ghost_map_array_tag_insert _ _ v_t nt l with "Htag_t_auth") as "[Ht Htag_t_auth]".
+  { intros i Hi. destruct (M_t !! (nt, l +ₗ i)) eqn:Hmt; last done.
+    destruct (Ht_dom nt (l +ₗ i) ltac:(eauto)) as (? & ?); congruence. }
+  iMod (ghost_map_array_tag_insert _ _ v_s nt l with "Htag_s_auth") as "[Hs Htag_s_auth]".
+  { intros i Hi. destruct (M_s !! (nt, l +ₗ i)) eqn:Hmt; last done.
+    destruct (Hs_dom nt (l +ₗ i) ltac:(eauto)) as (? & ?); congruence. }
+  iMod (ghost_map_array_tag_tk _ _ _ _ tk with "Ht") as "Ht".
+  iMod (ghost_map_array_tag_tk _ _ _ _ tk with "Hs") as "Hs".
+  set (M' := <[σ_t.(snp) := L]> M).
+  iPoseProof (ghost_map_lookup with "Hc Hcid") as "%HM_c".
+  iMod (ghost_map_update M' with "Hc Hcid") as "[Hc Hcid]".
+  iModIntro.
+  (* keep the persistent part if its public *)
+  iAssert (nt $$ tk ∗ if tk is tk_pub then nt $$ tk_pub else True)%I  with "[Hnt]" as "[$ Hpubt]".
+  { destruct tk; eauto. }
+  iExists v_t, v_s. iSplit; first done. iSplit; first done. iFrame "Ht Hs".
+
+  iAssert (⌜retag σ_t.(sst) σ_t.(snp) σ_t.(scs) c l ot FnEntry pk T = Some (Tagged nt, α', S (σ_t.(snp)))⌝)%I as "%Hretag_t".
+  { iPoseProof (state_rel_calls_eq with "Hsrel") as "<-".
+    iPoseProof (state_rel_stacks_eq with "Hsrel") as "<-".
+    subst nt. iPoseProof (state_rel_snp_eq with "Hsrel") as "<-". done. }
+  (* proving the value relation. TODO: duplicate  *)
+  iAssert (value_rel v_t v_s)%I as "#Hvrel"; last iFrame "Hvrel".
+  { iApply big_sepL2_forall; iSplit; first (iPureIntro;lia).
+    iIntros (i sc_t sc_s) "%Hs_t %Hs_v".
+    assert (i < tsize T)%nat as Hi. { rewrite -Hlen_t. eapply lookup_lt_is_Some_1. eauto. }
+    assert (Hsome_target : is_Some (σ_t.(shp) !! (l +ₗ i))).
+    { rewrite Hshp_t; last done. apply lookup_lt_is_Some_2. by rewrite Hlen_t. }
+    iPoseProof (state_rel_pub_if_not_priv _ _ _ _ _ _ (l +ₗ i) with "[] Hsrel [Hrel]") as "Hpub"; first done.
+    { iPoseProof (state_rel_calls_eq with "Hsrel") as "%Hcall_eq".
+      iPoseProof (state_rel_stacks_eq with "Hsrel") as "%Hstack_eq".
+      iPureIntro. intros t Hpriv.
+      eapply (priv_loc_UB_retag_access_eq σ_s σ_t); eauto; done. }
+    iPoseProof (pub_loc_lookup with "[] Hpub") as "(%sc_t' & %sc_s' & %Hread_both & Hsc_rel)"; first done.
+    enough (sc_t = sc_t' ∧ sc_s = sc_s') by naive_solver.
+    move : Hs_t Hs_v Hread_both (Hshp_s i Hi) (Hshp_t i Hi).
+    by move => -> -> [-> ->] [= ->] [= ->].
+  }
+
+  iFrame "Hcid". iSplitL "Hpubt".
+  { destruct mut; first done. iSplitR; first done. iRight.
+    iExists (σ_t.(snp)), (σ_t.(snp)). do 3 (iSplitR; first done). done. }
+
+  (* re-establishing the interpretation *)
+  iExists (<[c:=M']> M_call), (<[ nt := (tk, ()) ]> M_tag), (array_tag_map l nt v_t ∪ M_t), (array_tag_map l nt v_s ∪ M_s).
+  iFrame. iSplitL.
+  { (* state relation *)
+    rewrite /state_rel. simpl. iDestruct "Hsrel" as "(-> & %Hs_eq & -> & -> & -> & Hsrel)".
+    do 5 (iSplitL; first done). iIntros (l' Hsl').
+    iDestruct ("Hsrel" $! l' with "[//]") as "[Hpub | [%t' %Hpriv]]"; first (iLeft; iApply "Hpub").
+    iRight. iPureIntro. exists t'.
+    destruct Hpriv as (tk' & Hsome_tk' & Ht_l' & Htk'). exists tk'.
+    assert (t' ≠ nt). { intros ->. simplify_eq. }
+    rewrite lookup_insert_ne; last done.
+    split; first done. split.
+    - destruct Ht_l' as (sc0 & Ht_l'). exists sc0.
+      rewrite lookup_union_r; first done.
+      destruct (array_tag_map l nt v_t !! (t', l')) as [ a | ] eqn:Harr; last done.
+      specialize (array_tag_map_lookup1 l nt v_t t' l' ltac:(eauto)) as [Heq _]. congruence.
+    - destruct Htk' as [-> | [-> [c' Hin]]]; first by left. right. split; first done. exists c'.
+      destruct (decide (c' = c)) as [-> | Hneq].
+      + exists M'. rewrite lookup_insert; split; first done.
+        destruct Hin as (M'' & HM'' & (L' & HL' & Hin)). simplify_eq. exists L'.
+        rewrite lookup_insert_ne; done.
+      + destruct Hin as (M'' & HM'' & Hin). exists M''. rewrite lookup_insert_ne; done.
+  }
+  iSplitL.
+  { (* call interpretation. *)
+    iPureIntro. intros c' M''. destruct (decide (c' = c)) as [-> | Hneq].
+    - rewrite lookup_insert. intros [= <-]. simpl.
+      specialize (Hcall_interp c M HM_c) as (Hc & Hinterp). split; first done.
+      intros t S. subst M'. destruct (decide (t = σ_t.(snp))) as [-> | Hneq]; first last.
+      { rewrite lookup_insert_ne; last done. intros [Ht Hprot]%Hinterp. split; first lia.
+        intros l' Hl'. specialize (Hprot l' Hl') as (s & pm' & Hs & Hit & Hpm').
+        specialize (retag_item_active_preserving _ _ _ _ _ _ _ _ _ _ _ _ Hretag_t l' s (Tagged t) c pm' Hs Hc Hit) as (s' & -> & Hin'). eauto.
+      }
+      rewrite lookup_insert. intros [= <-]. split; first lia. subst L.
+      intros l'. rewrite seq_loc_set_elem. intros (i & Hi & ->).
+      eapply retag_fn_entry_item_active; done.
+    - (* TODO: duplication *)
+      rewrite lookup_insert_ne; last done. simpl. intros [Hc' HM']%Hcall_interp.
+      split; first done.
+      intros t' S HS. simpl. specialize (HM' t' S HS) as (Ht' & Hprot).
+      split; first lia. intros l' Hl'.
+      specialize (Hprot l' Hl') as (s & pm' & Hs & Hit & Hpm').
+      specialize (retag_item_active_preserving _ _ _ _ _ _ _ _ _ _ _ _ Hretag_t l' s (Tagged t') c' pm' Hs Hc' Hit) as (s' & -> & Hin'). eauto.
+  }
+  iSplitL.
+  { (* tag interpretation. *)
+    (* TODO: completely duplicated with the default lemma ... *)
+    iPoseProof (state_rel_get_pure with "Hsrel") as "%Hp".
+    destruct Hp as (Hsst & Hsnp & Hsnc & Hscs).
+    assert (∀l', M_t !! (nt, l') = None) as HMt_nt.
+    { intros l'. destruct (M_t !! (nt, l')) eqn:HM_t; last done.
+      specialize (Ht_dom nt l' ltac:(eauto)) as (? & ?); congruence. }
+    assert (∀l', M_s !! (nt, l') = None) as HMs_nt.
+    { intros l'. destruct (M_s !! (nt, l')) eqn:HM_s; last done.
+      specialize (Hs_dom nt l' ltac:(eauto)) as (? & ?); congruence. }
+    iPureIntro. split_and!.
+    { intros t tk'. rewrite lookup_insert_Some. intros [[<- [= <-]] | [Hneq Hsome_t]].
+      - cbn. split_and!; [lia | lia | | |].
+        + intros l' sc_t Ha%lookup_union_Some_l'; last done.
+          specialize (array_tag_map_lookup2 l nt v_t nt l' ltac:(eauto)) as [_ (i & Hi & ->)].
+          eapply retag_mut_loc_controlled; [ done | done | done | lia | ].
+          move : Ha. rewrite array_tag_map_lookup_Some; last done. move => <-. apply Hshp_t. lia.
+        + intros l' sc_s Ha%lookup_union_Some_l'; last done.
+          specialize (array_tag_map_lookup2 l nt v_s nt l' ltac:(eauto)) as [_ (i & Hi & ->)].
+          subst nt. rewrite -Hsnp. eapply retag_mut_loc_controlled; [ done | done | done | lia | ].
+          move : Ha. rewrite array_tag_map_lookup_Some; last done. move => <-. apply Hshp_s. lia.
+        + apply dom_agree_on_tag_union. { apply dom_agree_on_tag_array_tag_map. lia. }
+          apply dom_agree_on_tag_not_elem; done.
+      - cbn.
+        specialize (Htag_interp t tk' Hsome_t) as (Ht_t & Ht_s & Hcontrolled_t & Hcontrolled_s & Hagree).
+        split_and!; [ lia | lia | | | ].
+        + intros l' sc_t Ha. rewrite lookup_union_r in Ha; last by apply array_tag_map_lookup_None.
+          apply Hcontrolled_t in Ha.
+          eapply retag_loc_controlled_preserved; [done | done | | done | done].
+          intros <-. destruct tk'; [ done | | ]; move : Hsome_t Hpub; congruence.
+        + intros l' sc_s Ha. rewrite lookup_union_r in Ha; last by apply array_tag_map_lookup_None.
+          apply Hcontrolled_s in Ha.
+          eapply retag_loc_controlled_preserved; [done | done | | done | done].
+          intros <-. destruct tk'; [ done | | ]; move : Hsome_t Hpub; congruence.
+        + apply dom_agree_on_tag_union; last done.
+          apply dom_agree_on_tag_not_elem; apply array_tag_map_lookup_None; done.
+    }
+    { intros t l'.
+      rewrite lookup_union_is_Some lookup_insert_is_Some'. intros [[-> _]%array_tag_map_lookup2 | H%Ht_dom]; eauto. }
+    { intros t l'.
+      rewrite lookup_union_is_Some lookup_insert_is_Some'. intros [[-> _]%array_tag_map_lookup2 | H%Hs_dom]; eauto. }
+  }
+  done.
+Qed.
+
+Lemma sim_retag_fnentry mut T l_t l_s c M ot π Φ :
+  (0 < tsize T)%nat → (* for convenience: makes the proof easier *)
+  let pk : pointer_kind := RefPtr mut in
+  let pm := match mut with Mutable => Unique | Immutable => SharedReadOnly end in
+  let tk := match mut with Mutable => tk_unq | Immutable => tk_pub end in
+  (if mut is Immutable then is_freeze T else True) →
+  sc_rel (ScPtr l_t ot) (ScPtr l_s ot) -∗
+  c @@ M -∗
+  (∀ nt v_t v_s,
+    let L := seq_loc_set l_t (tsize T) in   (* uses that l_t = l_s *)
+    ⌜length v_t = tsize T⌝ -∗ ⌜length v_s = tsize T⌝ -∗
+    value_rel v_t v_s -∗  (*as the pointers were public before *)
+    c @@ <[nt := L]> M -∗
+    nt $$ tk -∗
+    l_t ↦t∗[tk]{nt} v_t -∗
+    l_s ↦s∗[tk]{nt} v_s -∗
+    (if mut is Immutable then sc_rel (ScPtr l_t (Tagged nt)) (ScPtr l_s (Tagged nt)) else True) -∗
+    #[ScPtr l_t (Tagged nt)] ⪯{π, Ω} #[ScPtr l_s (Tagged nt)] [{ Φ }]) -∗
+  Retag #[ScPtr l_t ot] #[ScCallId c] pk T FnEntry ⪯{π, Ω} Retag #[ScPtr l_s ot] #[ScCallId c] pk T FnEntry [{ Φ }].
+Proof.
+  intros Hsize pk pm tk Hmut. iIntros "#Hscrel Hcid Hsim".
+  iApply sim_lift_head_step_both. iIntros (??????) "((HP_t & HP_s & Hbor) & %Hthread & %Hsafe)".
+  (* exploit source to gain knowledge about stacks & that c is a valid id *)
+  specialize (pool_safe_irred _ _ _ _ _ _ _ Hsafe Hthread ltac:(done)) as (c' & ot' & l' & [= <- <-] & [= <-] & Hc_active & Hretag_some_s).
+  iPoseProof "Hscrel" as "(-> & _)".
+  iPoseProof (bor_interp_get_pure with "Hbor") as "%Hp".
+  have Hretag_some_t : is_Some (retag σ_t.(sst) σ_t.(snp) σ_t.(scs) c l_s ot FnEntry pk T).
+  { destruct Hp as (<- & <- & _ & <- & _). done. }
+  iModIntro. iSplitR.
+  { iPureIntro.
+    destruct Hretag_some_t as ([[] ] & Hretag_some_t).
+    do 3 eexists. eapply retag_head_step'; last done.
+    destruct Hp as (_ & _ & _ & <- & _). done.
+  }
+  iIntros (e_t' efs_t σ_t') "%Hhead_t".
+  specialize (head_retag_inv _ _ _ _ _ _ _ _ _ _ _ Hhead_t) as (nt & α' & nxtp' & Hretag_t & -> & -> & -> & Hc).
+  have Hretag_s : retag σ_s.(sst) σ_s.(snp) σ_s.(scs) c l_s ot FnEntry pk T = Some (nt, α', nxtp').
+  { destruct Hp as (-> & -> & _ & -> & _). done. }
+  assert (Hhead_s : head_step P_s (Retag #[ScPtr l_s ot] #[ScCallId c] pk T FnEntry) σ_s #[ScPtr l_s nt]%E (mkState (shp σ_s) α' (scs σ_s) nxtp' (snc σ_s)) []).
+  { eapply retag_head_step'; done. }
+  specialize (retag_change_ref_NZST _ _ _ _ _ _ _ _ _ _ _ _ Hsize Hretag_s) as [-> ->].
+
+  iPoseProof (bor_interp_get_state_wf with "Hbor") as "[%Hwf_t %Hwf_s]".
+  iMod (bor_interp_retag_fnentry _ _ _ _ _ _ _ _ _ Hretag_s with "Hscrel Hcid Hbor") as
+    (v_t v_s) "(%Hlen_t & %Hlen_s & Hval & Hcid & Htag & Ht & Hs & Hpub & Hbor)"; first done.
+  { destruct Hp as (_ & <- & _). eapply head_step_wf; eauto. }
+  { eapply head_step_wf; eauto. }
+  iModIntro.
+
+  iExists #[ScPtr l_s (Tagged σ_s.(snp))]%E, [], (mkState σ_s.(shp) α' σ_s.(scs) (S σ_s.(snp)) σ_s.(snc)).
+  iSplitR; first done.
+  destruct Hp as (_ & -> & _).
+  iFrame "Hbor HP_t HP_s".
+  iSplitL; last done.
+  iApply ("Hsim" with "[] [] Hval Hcid Htag Ht Hs Hpub"); [done | done | ..].
+Qed.
+
+(** Updates for calls sets *)
+(* TODO: maybe formulate that with [update_si] instead *)
+Lemma sim_protected_unprotectN M L l c t tk v_t v_s  π Φ e_t e_s :
+  (∀ i : nat, (i < length v_t)%nat → (l +ₗ i) ∈ L) →
+  M !! t = Some L →
+  c @@ M -∗
+  t $$ tk -∗
+  l ↦t∗[tk]{t} v_t -∗
+  l ↦s∗[tk]{t} v_s -∗
+  value_rel v_t v_s -∗
+  (c @@ (<[t := L ∖ (seq_loc_set l (length v_t)) ]> M) -∗ t $$ tk -∗ l ↦t∗[tk]{t} v_t -∗ l ↦s∗[tk]{t} v_s -∗ e_t ⪯{π, Ω} e_s [{ Φ }]) -∗
+  e_t ⪯{π, Ω} e_s [{ Φ }].
+Proof.
+  iIntros (Hl HL) "Hc Htag Ht Hs #Hvrel Hsim". 
+  iApply sim_update_si. rewrite /update_si. iIntros (?????) "(HP_t & HP_s & Hbor)".
+  set (L' := L ∖ seq_loc_set l (length v_t)). set (M' := <[ t := L' ]> M).
+  iPoseProof (value_rel_length with "Hvrel") as "%Hlen".
+  iPoseProof (heap_protected_readN_source with "Hbor Hs Htag Hc") as "(%Hv_s & % & %)".
+  { intros i Hi. exists L. split; first done. apply Hl. lia. } 
+  iPoseProof (heap_protected_readN_target with "Hbor Ht Htag Hc") as "(%Hv_t & % & %)".
+  { intros i Hi. exists L. split; first done. apply Hl. lia. } 
+
+  iDestruct "Hbor" as "(% & % & % & % & (Hcall_auth & Htag_auth & Htag_t_auth & Htag_s_auth) & #Hsrel & %Hcall_interp & %Htag_interp & %Hwf_s & %Hwf_t)". 
+  iPoseProof (ghost_map_lookup with "Hcall_auth Hc") as "%HcM".
+  iMod (ghost_map_update M' with "Hcall_auth Hc") as "[Hcall_auth Hc]".
+  iModIntro. iFrame "HP_t HP_s". iSplitR "Hsim Hc Ht Htag Hs"; last by iApply ("Hsim" with "Hc Htag Ht Hs").
+  iExists (<[ c := M' ]> M_call), M_tag, M_t, M_s. iFrame. 
+  iSplitL "Hsrel". 
+  { iDestruct "Hsrel" as "(%Hdom_eq & %Hsst_eq & %Hsnp_eq & %Hsnc_eq & %Hscs_eq & Hloc)". 
+    do 5 (iSplitR; first done).
+    iIntros (l' Hl'). iDestruct ("Hloc" $! l' with "[//]") as "[Hpub | %Hpriv]"; first by iLeft.
+    destruct (decide (l' ∈ seq_loc_set l (length v_t))) as [(i & Hi & ->)%seq_loc_set_elem | Hnotin]. 
+    - (* location is made public *)
+      iLeft. iIntros (sc_t' Hsc_t'). 
+      specialize (Hv_t i Hi) as Heq. rewrite Heq in Hsc_t'. 
+      iExists (v_s !!! i). iSplitR. 
+      + iPureIntro. rewrite Hv_s; last lia. apply list_lookup_lookup_total, lookup_lt_is_Some_2. lia. 
+      + iPoseProof (value_rel_lookup_total v_t v_s i with "Hvrel") as "Hsc"; first lia.
+        rewrite -(list_lookup_total_correct _ _ _ Hsc_t'). done.
+    - (* location is still private *)
+      iRight. iPureIntro. destruct Hpriv as (t' & tk' & Htk' & Hsome & Hpriv).
+      exists t', tk'. split; first done. split; first done. 
+      destruct Hpriv as [-> | [-> Hpriv]]; first by left. right; split; first done.
+      destruct Hpriv as (c' & M'' & Hc' & Hin').
+      destruct (decide (c' = c)) as [-> | Hneq]; first last.
+      { exists c', M''. rewrite lookup_insert_ne; done. } 
+      exists c, M'. rewrite lookup_insert. split; first done. 
+      destruct (decide (t' = t)) as [-> | Hneq']; first last. 
+      { destruct Hin' as (L'' & HL'' & Hl''). exists L''. split; last done. 
+        simplify_eq. rewrite lookup_insert_ne; done. 
+      } 
+      destruct Hin' as (L'' & HL'' & Hl''). exists L'. split; first by rewrite lookup_insert. 
+      simplify_eq. subst L'. apply elem_of_difference. done. 
+  } 
+  iSplitL; last done.
+  iPureIntro. intros c' M''. rewrite lookup_insert_Some. intros [[<- <-] | [Hneq Hsome]].
+  - apply Hcall_interp in HcM as [Hc HcM]. split; first done.
+    intros t' L''. subst M'. rewrite lookup_insert_Some. intros [[<- <-] | [Hneq' Hsome']].
+    + specialize (HcM t L HL) as (Ht & HsL). split; first done. 
+      intros l'. rewrite elem_of_difference. intros [Hl'%HsL _]. done. 
+    + specialize (HcM _ _ Hsome') as (Ht & HsL). done.
+  - apply Hcall_interp in Hsome as [Hc' Hsome]. done. 
+Qed.
+
+Lemma sim_protected_unprotect M L l c t tk sc_t sc_s π Φ e_t e_s :
+  l ∈ L →
+  M !! t = Some L →
+  c @@ M -∗
+  t $$ tk -∗
+  l ↦t[tk]{t} sc_t -∗
+  l ↦s[tk]{t} sc_s -∗
+  sc_rel sc_t sc_s -∗
+  (c @@ (<[t := L ∖ {[ l ]} ]> M) -∗ t $$ tk -∗ l ↦t[tk]{t} sc_t -∗ l ↦s[tk]{t} sc_s -∗ e_t ⪯{π, Ω} e_s [{ Φ }]) -∗
+  e_t ⪯{π, Ω} e_s [{ Φ }].
+Proof.
+  iIntros (Hin HL) "Hc Htag Ht Hs Hrel Hsim". 
+  iApply (sim_protected_unprotectN M L l c t tk [sc_t] [sc_s] with "Hc Htag [Ht] [Hs] [Hrel] [Hsim]"). 
+  - simpl. intros i Hi. replace i with O by lia. rewrite shift_loc_0_nat. done. 
+  - done. 
+  - iApply big_sepL_singleton. rewrite shift_loc_0_nat. done. 
+  - iApply big_sepL_singleton. rewrite shift_loc_0_nat. done. 
+  - iApply big_sepL2_singleton. done. 
+  - simpl. rewrite shift_loc_0_nat union_empty_r_L.
+    rewrite /array_tag !big_sepL_singleton !shift_loc_0_nat. done. 
+Qed.
+
+Lemma sim_remove_empty_calls t L M c e_t e_s π Φ : 
+  M !! t = Some L →
+  L = ∅ →
+  c @@ M -∗
+  (c @@ (delete t M) -∗ e_t ⪯{π, Ω} e_s [{ Φ }]) -∗
+  e_t ⪯{π, Ω} e_s [{ Φ }].
+Proof. 
+  iIntros (Ht ->) "Hc Hsim". 
+  iApply sim_update_si. rewrite /update_si. iIntros (?????) "(HP_t & HP_s & Hbor)".
+  set (M' := delete t M).
+  iDestruct "Hbor" as "(% & % & % & % & (Hcall_auth & Htag_auth & Htag_t_auth & Htag_s_auth) & #Hsrel & %Hcall_interp & %Htag_interp & %Hwf_s & %Hwf_t)". 
+  iPoseProof (ghost_map_lookup with "Hcall_auth Hc") as "%HcM".
+  iMod (ghost_map_update M' with "Hcall_auth Hc") as "[Hcall_auth Hc]".
+  iModIntro. iFrame "HP_t HP_s". iSplitR "Hsim Hc"; last by iApply ("Hsim" with "Hc").
+  iExists (<[ c := M' ]> M_call), M_tag, M_t, M_s. iFrame. 
+  iSplitL "Hsrel". 
+  { iDestruct "Hsrel" as "(%Hdom_eq & %Hsst_eq & %Hsnp_eq & %Hsnc_eq & %Hscs_eq & Hloc)". 
+    do 5 (iSplitR; first done).
+    iIntros (l' Hl'). iDestruct ("Hloc" $! l' with "[//]") as "[Hpub | %Hpriv]"; first by iLeft.
+    iRight. iPureIntro. destruct Hpriv as (t' & tk' & Htk' & Hsome & Hpriv).
+    exists t', tk'. split; first done. split; first done. 
+    destruct Hpriv as [-> | [-> Hpriv]]; first by left. right; split; first done.
+    destruct Hpriv as (c' & M'' & Hc' & Hin').
+    destruct (decide (c' = c)) as [-> | Hneq]; first last.
+    { exists c', M''. rewrite lookup_insert_ne; done. } 
+    exists c, M'. rewrite lookup_insert. split; first done. 
+    destruct (decide (t' = t)) as [-> | Hneq']; first last. 
+    { destruct Hin' as (L'' & HL'' & Hl''). exists L''. split; last done. 
+      simplify_eq. rewrite lookup_delete_ne; done. 
+    } 
+    exfalso. destruct Hin' as (L'' & HL'' & Hl''). simplify_eq. done.
+  } 
+  iSplitL; last done.
+  iPureIntro. intros c' M''. rewrite lookup_insert_Some. intros [[<- <-] | [Hneq Hsome]].
+  - apply Hcall_interp in HcM as [Hc HcM]. split; first done.
+    intros t' L''. subst M'. rewrite lookup_delete_Some. intros [Hneq' Hsome']. naive_solver. 
+  - apply Hcall_interp in Hsome as [Hc' Hsome]. done. 
+Qed.
+
+(** Write lemmas *)
+(* TODO: these lemmas are missing requirements on the well-taggedness of the written values! *)
+
+(* note: this is a new lemma. we do not care about relating the values - we only care for the source expression requiring that [t] is still on top!
+  TODO: can we make that more general/nicer?
+*)
+Lemma sim_write_unique_unprotected π l_t l_s t T v_t v_s v_t' v_s' Φ :
+  t $$ tk_unq -∗
+  l_t ↦t∗[tk_unq]{t} v_t -∗
+  l_s ↦s∗[tk_unq]{t} v_s -∗
+  (t $$ tk_unq -∗ l_t ↦t∗[tk_unq]{t} v_t' -∗ l_s ↦s∗[tk_unq]{t} v_s' -∗ #[☠] ⪯{π, Ω} #[☠] [{ Φ }]) -∗
+  Write (Place l_t (Tagged t) T) #v_t' ⪯{π, Ω} Write (Place l_s (Tagged t) T) #v_s' [{ Φ }].
+Proof.
+Admitted.
+
+Lemma target_write_local v_t v_t' T l t Ψ :
+  length v_t = tsize T →
+  length v_t' = tsize T →
+  t $$ tk_local -∗
+  l ↦t∗[tk_local]{t} v_t -∗
+  (l ↦t∗[tk_local]{t} v_t' -∗ t $$ tk_local -∗ target_red #[☠] Ψ)%E -∗
+  target_red (Write (Place l (Tagged t) T) #v_t') Ψ.
+Proof.
+Admitted.
+
+Lemma source_write_local v_s v_s' T l t Ψ π :
+  length v_s = tsize T →
+  length v_s' = tsize T →
+  t $$ tk_local -∗
+  l ↦s∗[tk_local]{t} v_s -∗
+  (l ↦s∗[tk_local]{t} v_s' -∗ t $$ tk_local -∗ source_red #[☠] π Ψ)%E -∗
+  source_red (Write (Place l (Tagged t) T) #v_s') π Ψ.
+Proof.
+Admitted.
+
+Lemma target_write_protected v_t v_t' T l t c M Ψ :
+  length v_t = tsize T →
+  length v_t' = tsize T →
+  (∀ i: nat, (i < tsize T)%nat → call_set_in M t (l +ₗ i)) →
+  c @@ M -∗
+  t $$ tk_unq -∗
+  l ↦t∗[tk_unq]{t} v_t -∗
+  (l ↦t∗[tk_unq]{t} v_t' -∗ c @@ M -∗ t $$ tk_unq -∗ target_red #[☠] Ψ)%E -∗
+  target_red (Write (Place l (Tagged t) T) #v_t') Ψ.
+Proof.
+Admitted.
+
+(* doesn't need protectors: if the item isn't there anymore, it will be UB *)
+Lemma source_write_unique v_s v_s' T l t Ψ π :
+  length v_s = tsize T →
+  length v_s' = tsize T →
+  t $$ tk_unq -∗
+  l ↦s∗[tk_unq]{t} v_s -∗
+  (l ↦s∗[tk_unq]{t} v_s' -∗ t $$ tk_unq -∗ source_red #[☠] π Ψ)%E -∗
+  source_red (Write (Place l (Tagged t) T) #v_s') π Ψ.
+Proof.
+Admitted.
+
+(** Copy lemmas *)
+Lemma target_copy_local v_t T l t Ψ :
+  length v_t = tsize T →
+  t $$ tk_local -∗
+  l ↦t∗[tk_local]{t} v_t -∗
+  (l ↦t∗[tk_local]{t} v_t -∗ t $$ tk_local -∗ target_red #v_t Ψ)%E -∗
+  target_red (Copy (Place l (Tagged t) T)) Ψ.
+Proof.
+  iIntros (Hlen) "Htag Ht Hsim".
+  iApply target_red_lift_head_step. iIntros (?????) "(HP_t & HP_s & Hbor)".
+  iModIntro.
+  iPoseProof (heap_local_readN_target with "Hbor Ht Htag") as "(%Hd & %Hstack & %Hwf)".
+  rewrite Hlen in Hd Hstack.
+  have READ_t : read_mem l (tsize T) σ_t.(shp) = Some v_t.
+  { apply read_mem_values'; done. }
+  iPoseProof (bor_interp_get_state_wf with "Hbor") as "[%Hwf_t %]".
+  have Eq_stk : memory_read σ_t.(sst) σ_t.(scs) l (Tagged t) (tsize T) = Some σ_t.(sst).
+  { apply memory_read_access1. intros i Hi.
+    specialize (Hstack i Hi). eexists; split; first done. eapply bor_state_own_access1_read; done. }
+  iSplitR.
+  { iPureIntro. do 3 eexists; eapply copy_head_step'; [done | done | eauto ]. }
+  iIntros (e_t' efs_t σ_t') "%Hhead".
+  specialize (head_copy_inv _ _ _ _ _ _ _ _ Hhead) as [-> [(v_t' & α' & READ & ACC & BOR & -> & ->) | (_ & Hfail & _)]]; last congruence.
+  rewrite READ in READ_t. simplify_eq.
+  iModIntro. iSplitR; first done.
+  iFrame "HP_t HP_s".
+  iSplitL "Hbor"; last iApply ("Hsim" with "Ht Htag").
+  destruct σ_t; done.
+Qed.
+
+
+Lemma source_copy_local v_s T l t Ψ π :
+  length v_s = tsize T →
+  t $$ tk_local -∗
+  l ↦s∗[tk_local]{t} v_s -∗
+  (l ↦s∗[tk_local]{t} v_s -∗ t $$ tk_local -∗ source_red #v_s π Ψ)%E -∗
+  source_red (Copy (Place l (Tagged t) T)) π Ψ.
+Proof.
+  iIntros (Hlen) "Htag Hs Hsim".
+  iApply source_red_lift_head_step. iIntros (??????) "[(HP_t & HP_s & Hbor) _]".
+  iModIntro.
+  iPoseProof (bor_interp_get_state_wf with "Hbor") as "[% %Hwf_s]".
+  iPoseProof (heap_local_readN_source with "Hbor Hs Htag") as "(%Hd & %Hstack & %Hwf)".
+  rewrite Hlen in Hd Hstack.
+  have READ_s : read_mem l (tsize T) σ_s.(shp) = Some v_s.
+  { apply read_mem_values'; done. }
+  have Eq_stk : memory_read σ_s.(sst) σ_s.(scs) l (Tagged t) (tsize T) = Some σ_s.(sst).
+  { apply memory_read_access1. intros i Hi.
+    specialize (Hstack i Hi). eexists; split; first done. eapply bor_state_own_access1_read; done. }
+  assert (head_reducible P_s (Copy (Place l (Tagged t) T)) σ_s) as (e_s' & σ_s' & efs & Hhead).
+  { do 3 eexists; eapply copy_head_step'; [done | done | eauto ]. }
+  iExists e_s', σ_s'.
+  specialize (head_copy_inv _ _ _ _ _ _ _ _ Hhead) as [-> [(v_t' & α' & READ & ACC & BOR & -> & ->) | (_ & Hfail & _)]]; last congruence.
+  rewrite READ in READ_s. simplify_eq.
+  iFrame "HP_t HP_s". iSplitR; first done.
+  iSplitL "Hbor"; last by iApply ("Hsim" with "Hs Htag"). iModIntro.
+  by destruct σ_s.
+Qed.
+
+(* should work for any tag_kind [tk] *)
+Lemma target_copy_protected v_t T l t tk Ψ c M  :
+  length v_t = tsize T →
+  (∀ i: nat, (i < tsize T)%nat → call_set_in M t (l +ₗ i)) →
+  c @@ M -∗
+  t $$ tk -∗
+  l ↦t∗[tk]{t} v_t -∗
+  (l ↦t∗[tk]{t} v_t -∗ c @@ M -∗ t $$ tk -∗ target_red #v_t Ψ)%E -∗
+  target_red (Copy (Place l (Tagged t) T)) Ψ.
+Proof.
+  iIntros (Hlen Hprotected) "Hcall Htag Ht Hsim".
+  iApply target_red_lift_head_step. iIntros (?????) "(HP_t & HP_s & Hbor)".
+  iModIntro.
+  iPoseProof (heap_protected_readN_target with "Hbor Ht Htag Hcall") as "(%Hd & %Hown & %Hwf)".
+  { by rewrite Hlen. }
+  rewrite Hlen in Hd Hown.
+  have READ_t : read_mem l (tsize T) σ_t.(shp) = Some v_t.
+  { apply read_mem_values'; done. }
+  iPoseProof (bor_interp_get_state_wf with "Hbor") as "[%Hwf_t %]".
+  have Eq_stk : memory_read σ_t.(sst) σ_t.(scs) l (Tagged t) (tsize T) = Some σ_t.(sst).
+  {
+    apply memory_read_access1. intros i Hi.
+    specialize (Hown i Hi). destruct (bor_state_own_some_stack _ _ _ _ Hown) as (stk & Hs_stk).
+    exists stk. split; first done. eapply bor_state_own_access1_read; done.
+  }
+  iSplitR.
+  { iPureIntro. do 3 eexists; eapply copy_head_step'; [done | eapply read_mem_values'; eauto | eauto]. }
+  iIntros (e_t' efs_t σ_t') "%Hhead".
+  specialize (head_copy_inv _ _ _ _ _ _ _ _ Hhead) as [-> [(v_t' & α' & READ & ACC & BOR & -> & ->) | (_ & Hfail & _)]]; last congruence.
+  rewrite READ in READ_t. simplify_eq.
+  iModIntro. iSplitR; first done.
+  iFrame "HP_t HP_s".
+  iSplitL "Hbor"; last iApply ("Hsim" with "Ht Hcall Htag").
+  destruct σ_t; done.
+Qed.
+
+(* Since copies without granting tags are not UB in the source but yield poison, 
+  we also need protection here to gain any knowledge about the value. *)
+Lemma source_copy_protected v_s T l t tk Ψ c M π :
+  length v_s = tsize T →
+  (∀ i: nat, (i < tsize T)%nat → call_set_in M t (l +ₗ i)) →
+  c @@ M -∗
+  t $$ tk -∗
+  l ↦s∗[tk]{t} v_s -∗
+  (l ↦s∗[tk]{t} v_s -∗ c @@ M -∗ t $$ tk -∗ source_red #v_s π Ψ)%E -∗
+  source_red (Copy (Place l (Tagged t) T)) π Ψ.
+Proof.
+  iIntros (Hlen Hprotected) "Hcall Htag Hs Hsim".
+  iApply source_red_lift_head_step. iIntros (??????) "[(HP_t & HP_s & Hbor) %Hsafe]".
+  iModIntro.
+  iPoseProof (heap_protected_readN_source with "Hbor Hs Htag Hcall") as "(%Hd & %Hown & %Hwf)".
+  { by rewrite Hlen. }
+  rewrite Hlen in Hd Hown.
+  have READ_t : read_mem l (tsize T) σ_s.(shp) = Some v_s.
+  { apply read_mem_values'; done. }
+  iPoseProof (bor_interp_get_state_wf with "Hbor") as "[% %Hwf_s]".
+  have Eq_stk : memory_read σ_s.(sst) σ_s.(scs) l (Tagged t) (tsize T) = Some σ_s.(sst).
+  {
+    apply memory_read_access1. intros i Hi.
+    specialize (Hown i Hi). destruct (bor_state_own_some_stack _ _ _ _ Hown) as (stk & Hs_stk).
+    exists stk. split; first done. eapply bor_state_own_access1_read; done.
+  }
+  iExists (#v_s)%E, _. 
+  iSplitR.
+  { iPureIntro. eapply copy_head_step'; [done | eapply read_mem_values'; eauto | eauto]. }
+  iModIntro. iFrame "HP_t HP_s".
+  iSplitL "Hbor"; last iApply ("Hsim" with "Hs Hcall Htag").
+  destruct σ_s; done.
+Qed.
+
+(* We can also read from unprotected source locations. 
+  But then we may get poison if the value isn't there anymore. *)
+Lemma source_copy_any v_s T l t tk Ψ π :
+  length v_s = tsize T →
+  t $$ tk -∗
+  l ↦s∗[tk]{t} v_s -∗
+  (∀ v_s', ⌜v_s' = v_s ∨ v_s' = replicate (length v_s) ScPoison⌝ -∗ l ↦s∗[tk]{t} v_s -∗ t $$ tk -∗ source_red #v_s' π Ψ)%E -∗
+  source_red (Copy (Place l (Tagged t) T)) π Ψ.
+Proof.
+Admitted. 
+
+(* TODO: define ghost state that does allow us to use a later source_copy to resolve the value *)
+Lemma target_copy_deferred v_t T l t tk Ψ :
+  length v_t = tsize T →
+  t $$ tk -∗
+  l ↦t∗[tk]{t} v_t -∗
+  (l ↦t∗[tk]{t} v_t -∗ t $$ tk -∗ target_red #v_t Ψ)%E -∗
+  target_red (Copy (Place l (Tagged t) T)) Ψ.
+Proof. 
+Abort.
+
+(* TODO: with the right ghost state, this should allow use to resolve "deferred" target copies *)
+Lemma source_copy_resolve_deferred v_s T l t Ψ tk π :
+  length v_s = tsize T →
+  t $$ tk -∗
+  l ↦s∗[tk]{t} v_s -∗
+  (l ↦s∗[tk]{t} v_s -∗ t $$ tk -∗ source_red #v_s π Ψ)%E -∗
+  source_red (Copy (Place l (Tagged t) T)) π Ψ.
+Proof.
+Abort.
+
+(** Alloc *)
+Lemma sim_alloc_local T Φ π :
+  (∀ t l, t $$ tk_local -∗
+    l ↦t∗[tk_local]{t} repeat ScPoison (tsize T) -∗
+    l ↦s∗[tk_local]{t} repeat ScPoison (tsize T) -∗
+    Place l (Tagged t) T ⪯{π, Ω} Place l (Tagged t) T [{ Φ }]) -∗
+  Alloc T ⪯{π, Ω} Alloc T [{ Φ }].
+Proof.
+  iIntros "Hsim".
+  iApply sim_lift_head_step_both. iIntros (??????) "[(HP_t & HP_s & Hbor) %Hsafe]".
+  iPoseProof (bor_interp_get_pure with "Hbor") as "%Hp".
+  iModIntro. iSplitR.
+  { iPureIntro. do 3 eexists. econstructor 2; econstructor. }
+  iIntros (e_t' efs_t σ_t') "%Hhead".
+  inv_head_step.
+  set (l_s := (fresh_block σ_s.(shp), 0)).
+  iMod (heap_local_alloc _ _ _ T with "Hbor") as "(Hbor & Htag & Htarget & Hsource)".
+  iModIntro.
+  iExists (Place l_s (Tagged (σ_t.(snp))) T), [], (mkState (init_mem l_s (tsize T) σ_s.(shp)) (init_stacks σ_s.(sst) l_s (tsize T) (Tagged σ_s.(snp))) σ_s.(scs) (S σ_s.(snp)) σ_s.(snc)).
+  iFrame. iSplitR.
+  { iPureIntro. destruct Hp as (_ & <- & _).  econstructor 2; econstructor. }
+  iSplitL; last by iApply big_sepL2_nil.
+  subst l l_s. rewrite (fresh_block_det σ_s σ_t); last apply Hp.
+  iApply ("Hsim" with "Htag Htarget Hsource").
+Qed.
+
+(* local ownership makes strong assertions: we also have to deallocate the corresponding ghost state. *)
+Lemma sim_free_local l t T v_t v_s Φ π : 
+  t $$ tk_local -∗ 
+  l ↦t∗[tk_local]{t} v_t -∗
+  l ↦s∗[tk_local]{t} v_s -∗ 
+  #[☠] ⪯{π, Ω} #[☠] [{ Φ }] -∗
+  Free (Place l (Tagged t) T) ⪯{π, Ω} Free (Place l (Tagged t) T) [{ Φ }].
+Proof. 
+Admitted.
+
+End lifting.
