theories/stacked_borrows/steps_refl.v
@@ -1,0 +1,720 @@
+From iris.proofmode Require Export tactics.
+From iris.bi.lib Require Import fractional.
+From iris.base_logic.lib Require Import ghost_map.
+From simuliris.base_logic Require Export gen_sim_prog.
+From simuliris.simulation Require Export slsls.
+From simuliris.simulation Require Import lifting.
+From iris.prelude Require Import options.
+From simuliris.stacked_borrows Require Import tkmap_view.
+From simuliris.stacked_borrows Require Export defs.
+From simuliris.stacked_borrows Require Import steps_progress steps_retag steps_inv.
+From simuliris.stacked_borrows Require Import heap.
+
+Section lifting.
+Context `{!sborG Σ}.
+Implicit Types P Q : iProp Σ.
+Implicit Types Φ : expr → expr → iProp Σ.
+Implicit Types σ σ_s σ_t : state.
+Implicit Types r r_s r_t : result.
+Implicit Types l : loc.
+Implicit Types f : fname.
+
+Context (Ω : result → result → iProp Σ).
+
+
+Lemma sim_alloc_public T Φ π :
+  (∀ t l, t $$ tk_pub -∗
+    rrel (PlaceR l (Tagged t) T) (PlaceR l (Tagged t) T) -∗
+    Place l (Tagged t) T ⪯{π, Ω} Place l (Tagged t) T [{ Φ }]) -∗
+  Alloc T ⪯{π, Ω} Alloc T [{ Φ }].
+Proof.
+Admitted.
+
+Lemma sim_free_public T_t T_s l_t l_s bor_t bor_s Φ π :
+  rrel (PlaceR l_t bor_t T_t) (PlaceR l_s bor_s T_s) -∗
+  #[☠] ⪯{π, Ω} #[☠] [{ Φ }] -∗
+  Free (Place l_t bor_t T_t) ⪯{π, Ω} Free (Place l_s bor_s T_s) [{ Φ }].
+Proof.
+  iIntros "[#Hscrel ->] Hsim".
+  iPoseProof (sc_rel_ptr_source with "Hscrel") as "[%Heq Hpub]". injection Heq as [= -> ->].
+  iApply sim_lift_head_step_both. iIntros (??????) "[(HP_t & HP_s & Hbor) %Hsafe]".
+  iModIntro.
+  destruct Hsafe as [Hpool Hsafe].
+  specialize (pool_safe_irred _ _ _ _ _ _  _ Hsafe Hpool ltac:(done)) as (Hdealloc_s & (α' & Hstack_s)).
+
+  iPoseProof (bor_interp_get_pure with "Hbor") as "%Hp".
+  destruct Hp as (Hsst_eq & Hsnp_eq & Hsnc_eq & Hscs_eq & Hwf_s & Hwf_t & Hdom_eq).
+  iSplitR.
+  { iPureIntro. do 3 eexists. eapply dealloc_head_step'; [done | |].
+    - intros m. rewrite -Hdealloc_s. rewrite -!elem_of_dom Hdom_eq. done.
+    - instantiate (1 := α'). rewrite -Hsst_eq -Hscs_eq. done.
+  }
+  iIntros (e_t' efs_t σ_t') "%Hhead_t".
+  specialize (head_free_inv _ _ _ _ _ _ _ _ Hhead_t) as (α'0 & Hstack_t & Hdealloc_t & -> & -> & ->).
+  iAssert (⌜α'0 = α'⌝)%I as "->".
+  { iPureIntro. move : Hstack_t Hstack_s. rewrite Hsst_eq Hscs_eq. congruence. }
+  iModIntro.
+  pose (σ_s' := (mkState (free_mem l_s (tsize T_s) σ_s.(shp)) α' σ_s.(scs) σ_s.(snp) σ_s.(snc))).
+  assert (Hhead_s : head_step P_s (Free (Place l_s bor_s T_s)) σ_s (ValR [☠]%S) σ_s' []).
+  { eapply dealloc_head_step'; eauto. }
+  iExists (#[☠])%E, [], σ_s'. iSplitR; first done.
+  iFrame "HP_t HP_s".
+  iSplitR "Hsim"; first last. { iSplitL; done. }
+
+  iDestruct "Hbor" as "(% & % & % & % & (Hc & Htag_auth & Htag_t_auth & Htag_s_auth) & #Hsrel & %Hcall_interp & %Htag_interp & _ & _)".
+
+  (* prove that it is a public location *)
+  iAssert (⌜untagged_or_public M_tag bor_s⌝)%I as %Hpub.
+  { iDestruct "Hscrel" as "[_ [[-> _] | (%t1 & %t2 & -> & -> & <- & _)]]"; first done.
+    iPoseProof (tkmap_lookup with "Htag_auth Hpub") as "%". done.
+  }
+
+  (* we keep the head_step hypotheses to use the [head_step_wf] lemma below *)
+  (* re-establish the invariants *)
+  iExists M_call, M_tag, M_t, M_s.
+  iFrame "Hc Htag_auth Htag_t_auth Htag_s_auth".
+  iSplit; last iSplit; last iSplit; last iSplit.
+  - (* re-establish the state relation *)
+    admit. 
+  - (* re-establish the call set interpretation *)
+    admit.
+  - (* re-establish the tag interpretation *)
+    admit.
+  - iPureIntro. by eapply head_step_wf.
+  - iPureIntro. by eapply head_step_wf.
+Admitted.
+
+
+Lemma sim_copy_public_controlled_update σ l l' (bor : tag) (T : type) (α' : stacks) (t : ptr_id) (tk : tag_kind) sc :
+  memory_read σ.(sst) σ.(scs) l bor (tsize T) = Some α' →
+  state_wf σ →
+  (bor = Tagged t → tk = tk_pub) →
+  loc_controlled l' t tk sc σ →
+  loc_controlled l' t tk sc (mkState σ.(shp) α' σ.(scs) σ.(snp) σ.(snc)).
+Proof.
+  intros Hread Hwf Hbor Hcontrol Hpre.
+  (* need to update the loc_controlled.
+    intuitive justification:
+    - if l is not affected by the Copy, we are fine.
+    - if it is affected, we already know that we accessed with a public tag [bor_s].
+      In case this current tag [t] is local, we have a contradiction as the tags must be the same.
+      In case this current tag [t] is unique: if the item is in the stack, then it must still be because it would have been protected
+      In case this current tag [t] is public: it should still be there, as it is not incompatible with our copy access (we leave SharedROs there).
+  *)
+
+  specialize (for_each_access1 _ _ _ _ _ _ _ Hread) as Hsub.
+  assert (bor_state_pre l' t tk σ) as H.
+  { move : Hpre. destruct tk; [ | | done ].
+    all: intros (st' & pm & opro & Hα'_some & Hit & Hpm);
+      specialize (Hsub _ _ Hα'_some) as (st & Hα_some & Hsublist & _);
+      exists st, pm, opro;
+      split_and!; [ done | | done]; specialize (Hsublist _ Hit) as ([] & Hit' & Heq & Heq' & Hperm'); simpl in *;
+      rewrite Heq Heq' -Hperm'; done.
+  }
+  specialize (Hcontrol H) as [Hown Hmem].
+  split; last done.
+  move: Hpre.
+  destruct tk; simpl.
+  * (* goal: use access1_active_SRO_preserving *)
+    intros (st & pm & opro & Hsome_st & Hit & Hpm). exists st. split; first done.
+    destruct Hown as (st'' & Hsome_st'' & Hactive).
+    destruct (for_each_lookup_case _ _ _ _ _ Hread _ _ _ Hsome_st'' Hsome_st) as [-> | [Hacc _]]; first done.
+    destruct access1 as [ [n st']| ] eqn:Hacc_eq; simpl in Hacc; simplify_eq.
+    eapply access1_active_SRO_preserving; [ | done | apply Hacc_eq | done ].
+    eapply Hwf; done.
+  * intros (st & pm & opro & Hsome_st & Hit & Hpm).
+    destruct Hown as (st' & Hsome_st' & opro' & st'0 & Heq).
+    destruct (for_each_lookup_case _ _ _ _ _ Hread _ _ _ Hsome_st' Hsome_st) as [-> | [Hacc _]]; first by eauto.
+    destruct access1 as [ [n st'']| ] eqn:Hacc_eq; simpl in Hacc; simplify_eq.
+    exists st. split; first done. exists opro'.
+    eapply access1_head_preserving; [ eapply Hwf; done| done | | apply Hacc_eq| eexists; done ].
+    (* need that opro = opro' *)
+    specialize (access1_read_eq _ _ _ _ t _ _ _ ltac:(eapply Hwf; done) Hacc_eq ltac:(by left) Hit Hpm ltac:(done) ltac:(done)) as Heq.
+    simplify_eq. done.
+  * intros _. simpl in Hown.
+    specialize (for_each_access1_lookup_inv _ _ _ _ _ _ _ Hread _ _ Hown) as (st' & Hst' & [[n' Hacc_eq] | Heq]).
+    2: { rewrite Heq. done. }
+    specialize (access1_in_stack _ _ _ _ _ _ Hacc_eq) as (it & ->%elem_of_list_singleton & Htg & _).
+    (* contradiction, since t is public *)
+    simpl in Htg. subst bor. discriminate Hbor. done.
+Qed.
+
+Lemma sim_copy_public Φ π l_t bor_t T_t l_s bor_s T_s :
+  rrel (PlaceR l_t bor_t T_t) (PlaceR l_s bor_s T_s) -∗
+  (∀ v_t v_s, value_rel v_t v_s -∗ v_t ⪯{π, Ω} ValR v_s [{ Φ }]) -∗
+  Copy (PlaceR l_t bor_t T_t) ⪯{π, Ω} Copy (PlaceR l_s bor_s T_s) [{ Φ }].
+Proof.
+  iIntros "#Hrel Hsim".
+  iApply sim_lift_head_step_both. iIntros (??????) "[(HP_t & HP_s & Hbor) %Hsafe]".
+  iModIntro.
+  iDestruct "Hrel" as "[[<- Hrel] <-]".
+  iDestruct "Hbor" as "(% & % & % & % & (Hc & Htag_auth & Htag_t_auth & Htag_s_auth) & #Hsrel & %Hcall_interp & %Htag_interp & %Hwf_s & %Hwf_t)".
+  iPoseProof (state_rel_stacks_eq with "Hsrel") as "%Hstacks_eq".
+  iPoseProof (state_rel_calls_eq with "Hsrel") as "%Hcalls_eq".
+
+  (* prove that it is a public location *)
+  iAssert (⌜untagged_or_public M_tag bor_t ∧ bor_t = bor_s⌝)%I as %Hpub.
+  { iDestruct "Hrel" as "[[-> ->] | (%t1 & %t2 & -> & -> & <- & Hpub)]"; first done.
+    iPoseProof (tkmap_lookup with "Htag_auth Hpub") as "%". done.
+  }
+  destruct Hpub as [Hpub ->].
+
+  destruct Hsafe as [Hpool Hsafe].
+  specialize (pool_safe_irred _ _ _ _ _ _  _ Hsafe Hpool ltac:(done)) as [(v_s & Hread_s & (α' & Hstack_s) & Hwell_tagged_s) | Hfail]; first last. 
+  { (* failing copy *)
+    iSplitR. 
+    { iPureIntro. do 3 eexists. eapply failed_copy_head_step'; first done. 
+      rewrite -Hstacks_eq -Hcalls_eq. done. 
+    } 
+    iIntros (e_t' efs_t σ_t') "%Hhead_t".
+    specialize (head_copy_inv _ _ _ _ _ _ _ _ Hhead_t) as [-> [(? & ? & _ & ? & _) | (-> & ? & ->)]]; first congruence. 
+    iModIntro.
+    assert (Hhead_s : head_step P_s (Copy (Place l_t bor_s T_t)) σ_s (Val $ replicate (tsize T_t) ScPoison) σ_s []).
+    { eapply failed_copy_head_step'; eauto. }
+    iExists (Val $ replicate (tsize T_t) ScPoison), [], σ_s. iSplitR; first done.
+    iFrame. iSplitR "Hsim"; first last. 
+    { iSplitL; last done. iApply "Hsim". 
+      generalize (tsize T_t) => n. iInduction n as [ | n] "IH"; first by iApply big_sepL2_nil. 
+      rewrite /value_rel big_sepL2_cons; iFrame "IH". done. 
+    } 
+    iExists M_call, M_tag, M_t, M_s. iFrame. repeat (iSplit; done).
+  } 
+  (* successful copy *)
+  iAssert (⌜∀ i : nat, (i < tsize T_t)%nat → is_Some (shp σ_t !! (l_t +ₗ i))⌝)%I as "%Hsome_target".
+  { iPoseProof (state_rel_heap_lookup_Some with "Hsrel") as "%Hl".
+    iPureIntro. (* use read_mem_is_Some' *)
+    specialize (proj2 (read_mem_is_Some' l_t (tsize T_t) σ_s.(shp)) ltac:(eauto)) as Him.
+    intros i Hi. apply Hl, elem_of_dom. by eapply Him.
+  }
+
+
+  (* prove reducibility *)
+  iSplitR.
+  { iPoseProof (state_rel_dom_eq with "Hsrel") as "%Hdom".
+    iPureIntro.
+    destruct (read_mem_is_Some l_t (tsize T_t) σ_t.(shp)) as [v_t Eqvt].
+    { intros m. rewrite Hdom. apply (read_mem_is_Some' l_t (tsize T_t) σ_s.(shp)). by eexists. }
+    have Eqα'2: memory_read σ_t.(sst) σ_t.(scs) l_t bor_s (tsize T_t) = Some α'.
+    { rewrite -Hstacks_eq -Hcalls_eq. done. }
+    eexists; eexists; eexists. eapply copy_head_step'; eauto.
+  }
+  (* we keep the head_step hypotheses to use the [head_step_wf] lemma below *)
+  iIntros (e_t' efs_t σ_t') "%Hhead_t".
+  specialize (head_copy_inv _ _ _ _ _ _ _ _ Hhead_t) as [-> [(v_t & α'0 & COPY & ACC & BOR & -> & ->) | (-> & ? & ->)]]; last congruence. 
+  iAssert (⌜α'0 = α'⌝)%I as "->".
+  { iPureIntro. move : ACC Hstack_s. rewrite Hcalls_eq Hstacks_eq. congruence. }
+  iModIntro.
+  pose (σ_s' := (mkState (shp σ_s) α' (scs σ_s) (snp σ_s) (snc σ_s))).
+  assert (Hhead_s : head_step P_s (Copy (Place l_t bor_s T_t)) σ_s (ValR v_s) σ_s' []).
+  { eapply copy_head_step'; eauto. }
+  iExists (Val v_s), [], σ_s'. iSplitR; first done.
+  iFrame "HP_t HP_s".
+
+  iSplitR "Hsim".
+  {
+    (* re-establish the invariants *)
+    iExists M_call, M_tag, M_t, M_s.
+    iFrame "Hc Htag_auth Htag_t_auth Htag_s_auth".
+    iSplit; last iSplit; last iSplit; last iSplit.
+    - (* state rel *)
+      iPoseProof (state_rel_dom_eq with "Hsrel") as "%Hdom".
+      iPoseProof (state_rel_snp_eq with "Hsrel") as "%Hsnp".
+      iPoseProof (state_rel_snc_eq with "Hsrel") as "%Hsnc".
+      iSplit; first done. iSplit; first done. iSplit; first done.
+      iSplit; first done. iSplit; first done.
+      simpl. iIntros (l) "Hs". iPoseProof (state_rel_pub_or_priv with "Hs Hsrel") as "$".
+    - (* call invariant *)
+      iPureIntro. intros c M' HM'_some.
+      specialize (Hcall_interp c M' HM'_some) as (Hin & Hprot).
+      split; first by apply Hin. intros pid L HL_some. specialize (Hprot pid L HL_some) as [Hpid Hprot].
+      split; first by apply Hpid. intros l Hin_l.
+      specialize (Hprot l Hin_l) as (stk & pm & Hstk_some & Hin_stack & Henabled).
+      (* we use that reads must preserve active protectors (but note that the stack may have changed, even when there is an active protector) *)
+      specialize (for_each_access1_active_preserving _ _ _ _ _ _ _ ACC l stk Hstk_some) as (stk' & Hstk'_some & Hac_pres).
+      exists stk', pm. split; last split; [ done | by apply Hac_pres| done ].
+    - (* tag invariant *)
+      iPureIntro. destruct Htag_interp as (Htag_interp & Ht_dom & Hs_dom). split_and!; [ | done..].
+      intros t tk Htk_some. destruct (Htag_interp t tk Htk_some) as (Hsnp_lt_t & Hsnp_lt_s & Hctrl_t & Hctrl_s & Hag).
+      split_and!; [ done | done | | | done ].
+      + intros l sc_t Hsc_t. eapply sim_copy_public_controlled_update; [ by eauto .. | | by eauto].
+        intros ->. rewrite Hpub in Htk_some. congruence.
+      + intros l sc_s Hsc_s. eapply sim_copy_public_controlled_update; [ by eauto .. | | by eauto].
+        intros ->. rewrite Hpub in Htk_some. congruence.
+    - (* source state wf *)
+      iPureIntro. eapply head_step_wf; done.
+    - (* target state wf *)
+      iPureIntro. eapply head_step_wf; done.
+  }
+  iSplitL; last done.
+
+  iApply "Hsim".
+  (* proving the value relation *)
+  specialize (read_mem_values _ _ _ _ COPY) as [Hlen_t Hv_t].
+  specialize (read_mem_values _ _ _ _ Hread_s) as [Hlen_s Hv_s].
+
+  iApply big_sepL2_forall; iSplit; first (iPureIntro;lia).
+  iIntros (i sc_t sc_s) "%Hs_t %Hs_v".
+  assert (i < tsize T_t)%nat as Hi. { rewrite -Hlen_t. eapply lookup_lt_is_Some_1. eauto. }
+  iPoseProof (state_rel_pub_if_not_priv _ _ _ _ _ _ (l_t +ₗ i) with "[] Hsrel [Hrel]") as "Hpub".
+  { iPureIntro. by apply Hsome_target. }
+  { iPoseProof (state_rel_calls_eq with "Hsrel") as "%Hcall_eq".
+    iPoseProof (state_rel_stacks_eq with "Hsrel") as "%Hstack_eq".
+    iPureIntro. intros t Hpriv.
+    specialize (for_each_lookup_case_2 _ _ _ _ _ Hstack_s) as (Hstk & _).
+    specialize (Hstk i%nat ltac:(lia)) as (stk & stk' & ? & (_ & Haccess_some)).
+    eapply (priv_pub_access_UB _ AccessRead _ _ _ _ stk); [ | | apply Hpriv | eauto..].
+    - rewrite -Hstack_eq. done.
+    - move : Haccess_some. rewrite Hcall_eq. destruct access1; cbn; intros; simplify_eq. eauto.
+  }
+  iPoseProof (pub_loc_lookup with "[] Hpub") as "(%sc_t' & %sc_s' & %Hread_both & Hsc_rel)"; first by eauto.
+  enough (sc_t = sc_t' ∧ sc_s = sc_s') by naive_solver.
+  move : Hread_both (Hv_t i Hi) (Hv_s i Hi) Hs_t Hs_v.
+  by move => [-> ->] <- <- [= ->] [= ->].
+Qed.
+
+(** Write *)
+Lemma loc_controlled_write_public σ bor tk l l' T α' sc v t :
+  state_wf σ →
+  (bor = Tagged t → tk = tk_pub) →
+  memory_written σ.(sst) σ.(scs) l' bor (tsize T) = Some α' →
+  length v = tsize T →
+  loc_controlled l t tk sc σ →
+  loc_controlled l t tk sc (mkState (write_mem l' v σ.(shp)) α' σ.(scs) σ.(snp) σ.(snc)).
+Proof.
+  rewrite /loc_controlled //= => Hwf Hpub Hstack Hlen Hcontrol.
+  destruct (write_mem_lookup_case l' v σ.(shp) l) as [(i & Hi & -> & Hwrite_i) | (Hi & ->)];
+      first last.
+  { (* l is NOT written to *)
+    destruct (for_each_lookup _ _ _ _ _ Hstack) as (_ & _ & Hstack_eq).
+    rewrite /bor_state_pre /bor_state_own. rewrite !Hstack_eq. 2: intros; apply Hi; lia.
+    apply Hcontrol.
+  }
+  (* considering one of the written-to locations *)
+  intros Hpre.
+  specialize (for_each_access1 _ _ _ _ _ _ _ Hstack) as Hsub.
+  destruct Hcontrol as (Hown & Hmem).
+  { destruct tk; simpl in *; [ | | done].
+    all: destruct Hpre as (stk & pm & opro & (stk' & -> & Hsubl & _)%Hsub & Hit & Hpm).
+    all: apply Hsubl in Hit as ([pm' tg' opro'] & Hit2 & Htg & Hprot & Hperm).
+    all: exists stk', pm', opro'; simpl in *; rewrite Htg.
+    all:  split_and!; [done | done | rewrite Hperm; done].
+  }
+  (* we now lead this to a contradiction: the write was UB/the tags are contradictory *)
+  specialize (for_each_lookup _ _ _ _ _ Hstack) as (Ha & _).
+  destruct tk; simpl in *.
+  * (* public *)
+    destruct Hpre as (stk' & pm & opro & Hstk' & Hit & Hpm).
+    exfalso. destruct Hown as (stk & Hstk & Hactive).
+    specialize (Ha i _ ltac:(lia) Hstk) as (stk'' & Hstk'' & Hacc).
+    destruct access1 as [[n ?] | ] eqn:Hacc_eq; last done. injection Hacc as [= ->].
+    simplify_eq.
+    eapply access1_write_remove_incompatible_active_SRO; [ | done | apply Hacc_eq | done ].
+    by eapply Hwf.
+  * (* unique *)
+    destruct Hpre as (stk' & pm & opro & Hstk' & Hit & Hpm).
+    exfalso. destruct Hown as (stk & Hstk & Hprot).
+    specialize (Ha i _ ltac:(lia) Hstk) as (stk'' & Hstk'' & Hacc).
+    destruct access1 as [[n ?] | ] eqn:Hacc_eq; last done. injection Hacc as [= ->].
+    simplify_eq.
+    destruct Hprot as (opro' & stk'' & ->).
+    eapply access1_write_remove_incompatible_head;
+      [ | eexists; eexists; reflexivity | apply Hacc_eq | | done].
+    { by eapply Hwf. }
+    (* contradiction, since t is public *)
+    intros <-. discriminate Hpub. done.
+  * (* local *)
+    exfalso.
+    specialize (Ha i _ ltac:(lia) Hown) as (stk'' & Hstk'' & Hacc).
+    destruct access1 as [[n ?] | ] eqn:Hacc_eq; last done. injection Hacc as [= ->].
+    specialize (access1_in_stack _ _ _ _ _ _ Hacc_eq) as (it & ->%elem_of_list_singleton & Htg & _).
+    (* contradiction, since t is public *)
+    simpl in Htg. subst bor. discriminate Hpub. done.
+Qed.
+
+Lemma sim_write_public Φ π l_t bor_t T_t l_s bor_s T_s v_t' v_s' :
+  rrel (PlaceR l_t bor_t T_t) (PlaceR l_s bor_s T_s) -∗
+  value_rel v_t' v_s' -∗
+  (#[☠] ⪯{π, Ω} #[☠] [{ Φ }]) -∗
+  Write (Place l_t bor_t T_t) v_t' ⪯{π, Ω} Write (Place l_s bor_s T_s) v_s' [{ Φ }].
+Proof.
+  iIntros "Hrel #Hvrel Hsim". iDestruct "Hrel" as "[#Hscrel ->]".
+  iPoseProof (sc_rel_ptr_source with "Hscrel") as "[%Heq Hpub]". injection Heq as [= -> ->].
+  iApply sim_lift_head_step_both. iIntros (??????) "[(HP_t & HP_s & Hbor) %Hsafe]".
+  iModIntro.
+  destruct Hsafe as [Hpool Hsafe].
+  specialize (pool_safe_irred _ _ _ _ _ _  _ Hsafe Hpool ltac:(done)) as (Hread_s & (α' & Hstack_s) & Hwell_tagged_s & Hlen_s').
+  iPoseProof (value_rel_length with "Hvrel") as "%Hlen_t'".
+  iPoseProof (value_rel_tag_values_included_iff with "Hvrel") as "%Htag_included".
+
+  iPoseProof (bor_interp_get_pure with "Hbor") as "%Hp".
+  destruct Hp as (Hsst_eq & Hsnp_eq & Hsnc_eq & Hscs_eq & Hwf_s & Hwf_t & Hdom_eq).
+  iSplitR.
+  { iPureIntro. do 3 eexists. eapply write_head_step'; [lia | | |].
+    - rewrite -Hsnp_eq. apply Htag_included. done.
+    - rewrite -Hdom_eq. intros n Hn. apply Hread_s. lia.
+    - instantiate (1 := α'). rewrite -Hsst_eq -Hscs_eq. done.
+  }
+  iIntros (e_t' efs_t σ_t') "%Hhead_t".
+  specialize (head_write_inv _ _ _ _ _ _ _ _ _ Hhead_t) as (α'0 & -> & -> & -> & _ & Hin_dom & Hstack_t & Hwell_tagged_t).
+  iAssert (⌜α'0 = α'⌝)%I as "->".
+  { iPureIntro. move : Hstack_t Hstack_s. rewrite Hsst_eq Hscs_eq. congruence. }
+  iModIntro.
+  pose (σ_s' := (mkState (write_mem l_s v_s' σ_s.(shp)) α' σ_s.(scs) σ_s.(snp) σ_s.(snc))).
+  assert (Hhead_s : head_step P_s (Write (Place l_s bor_s T_s) v_s') σ_s (ValR [☠]%S) σ_s' []).
+  { eapply write_head_step'; eauto. intros. rewrite Hdom_eq. apply Hin_dom. lia. }
+  iExists (#[☠])%E, [], σ_s'. iSplitR; first done.
+  iFrame "HP_t HP_s".
+  iSplitR "Hsim"; first last. { iSplitL; done. }
+
+  iDestruct "Hbor" as "(% & % & % & % & (Hc & Htag_auth & Htag_t_auth & Htag_s_auth) & #Hsrel & %Hcall_interp & %Htag_interp & _ & _)".
+
+  (* prove that it is a public location *)
+  iAssert (⌜untagged_or_public M_tag bor_s⌝)%I as %Hpub.
+  { iDestruct "Hscrel" as "[_ [[-> _] | (%t1 & %t2 & -> & -> & <- & _)]]"; first done.
+    iPoseProof (tkmap_lookup with "Htag_auth Hpub") as "%". done.
+  }
+
+  (* we keep the head_step hypotheses to use the [head_step_wf] lemma below *)
+  (* re-establish the invariants *)
+  iExists M_call, M_tag, M_t, M_s.
+  iFrame "Hc Htag_auth Htag_t_auth Htag_s_auth".
+  iSplit; last iSplit; last iSplit; last iSplit.
+  - (* state rel *)
+    rewrite /state_rel; simpl. iSplitL.
+    { iPureIntro. apply gset_leibniz. rewrite !write_mem_dom; [by rewrite Hdom_eq | done..]. }
+    do 4 (iSplitL; first done). iDestruct "Hsrel" as "(_ & _ & _ & _ & _ & Hsrel)".
+    iIntros (l) "%Hs".
+    specialize (write_mem_lookup l_s v_s' σ_s.(shp)) as (Heq & Heq').
+    specialize (write_mem_lookup_case l_s v_t' σ_t.(shp) l) as [(i & Hi & -> & Hwrite) | (Hi & Hwrite)].
+    + (* we wrote to the location, and the written values must be related *)
+      iLeft. iIntros (sc_t Hsc_t). simpl in Hsc_t. rewrite Heq; last lia.
+      iExists (v_s' !!! i). rewrite Hwrite in Hsc_t.
+      rewrite -(list_lookup_total_correct _ _ _ Hsc_t).
+      iSplitR. { iPureIntro. apply list_lookup_lookup_total. apply lookup_lt_is_Some_2. lia. }
+      iApply (value_rel_lookup_total with "Hvrel"). lia.
+    + (* unaffected location *)
+      simpl. rewrite Hwrite in Hs.
+      iDestruct ("Hsrel" $! l with "[//]") as "[Hpubl | Hprivl]"; last by iRight.
+      iLeft. rewrite /pub_loc Hwrite Heq'; first done. intros. apply Hi. lia.
+  - (* call invariant *)
+    iPureIntro. intros c M' HM'_some. simpl.
+    specialize (Hcall_interp c M' HM'_some) as (Hin & Hprot).
+    split; first done. intros t L [Ht HL]%Hprot. split; first done.
+    intros l (stk & pm & Hsome_stk & Hit & Hpm)%HL.
+    specialize (for_each_access1_active_preserving _ _ _ _ _ _ _ Hstack_t _ _ Hsome_stk) as (stk' & Hstk'_some & Hac_pres).
+    exists stk', pm. split; last split; [ done | by apply Hac_pres| done ].
+  - (* tag invariant *)
+    iPureIntro. destruct Htag_interp as (Htag_interp & Ht_dom & Hs_dom). split_and!; [ | done..].
+    intros t tk Ht.
+    specialize (Htag_interp _ _ Ht) as (? & ? & Hcontrolled_t & Hcontrolled_s & Hdom).
+    split_and!; [ done | done | | | done ].
+    + intros l sc_t Hcontrol%Hcontrolled_t.
+      eapply loc_controlled_write_public; [ apply Hwf_t | | apply Hstack_t| lia | done].
+      intros ->. rewrite Hpub in Ht. congruence.
+    + intros l sc_s Hcontrol%Hcontrolled_s.
+      eapply loc_controlled_write_public; [ apply Hwf_s | | apply Hstack_s| lia | done].
+      intros ->. rewrite Hpub in Ht. congruence.
+  - (* source state wf *)
+    iPureIntro. eapply head_step_wf; done.
+  - (* target state wf *)
+    iPureIntro. eapply head_step_wf; done.
+Qed.
+
+(** Retag *)
+Lemma bor_interp_retag_public σ_s σ_t c l ot rkind kind T nt α' nxtp' :
+  retag σ_s.(sst) σ_s.(snp) σ_s.(scs) c l ot rkind kind T = Some (nt, α', nxtp') →
+  state_wf (mkState σ_t.(shp) α' σ_t.(scs) nxtp' σ_t.(snc)) →   (* could remove that assumption *)
+  state_wf (mkState σ_s.(shp) α' σ_s.(scs) nxtp' σ_s.(snc)) →   (* could remove that assumption *)
+  sc_rel (ScPtr l ot) (ScPtr l ot) -∗
+  bor_interp sc_rel σ_t σ_s ==∗
+  sc_rel (ScPtr l nt) (ScPtr l nt) ∗
+  bor_interp sc_rel (mkState σ_t.(shp) α' σ_t.(scs) nxtp' σ_t.(snc)) (mkState σ_s.(shp) α' σ_s.(scs) nxtp' σ_s.(snc)).
+Proof.
+  intros Hretag Hwf_t' Hwf_s'.
+  iIntros "Hscrel Hbor". iDestruct "Hbor" as "(% & % & % & % & (Hc & Htag_auth & Htag_t_auth & Htag_s_auth) & #Hsrel & %Hcall_interp & %Htag_interp & %Hwf_s & %Hwf_t)".
+
+  iDestruct "Hscrel" as "[_ #Hrel]".
+  iAssert (⌜untagged_or_public M_tag ot⌝)%I as %Hpub.
+  { iDestruct "Hrel" as "[[-> _] | (%t1 & %t2 & -> & -> & <- & Hpub)]"; first done.
+    iPoseProof (tkmap_lookup with "Htag_auth Hpub") as "%". done.
+  }
+
+  (* allocate resources *)
+  set (M_tag' := if decide (ot = nt) then M_tag else if nt is Tagged nt then <[nt := (tk_pub, ())]> M_tag else M_tag).
+  specialize (retag_change_nxtp _ _ _ _ _ _ _ _ _ _ _ _ Hretag) as Hle.
+  specialize (retag_change_tag _ _ _ _ _ _ _ _ _ _ _ _ Hretag) as Hnt.
+  iAssert (|==> (if decide (ot = nt) then True%I else if nt is Tagged nt then nt $$ tk_pub else True%I) ∗ tkmap_auth tag_name 1 M_tag')%I with "[Htag_auth]" as "Hnt".
+  { destruct (decide (ot = nt)) as [ | Hneq]; first by eauto.
+    destruct Hnt as [ -> | Hnt]; first done.
+    destruct nt as [ nt | ]; last by eauto. destruct Hnt as [-> ->].
+    iMod (tkmap_insert tk_pub σ_s.(snp) tt with "Htag_auth") as "[$ $]"; last done.
+    destruct (M_tag !! snp σ_s) as [ [? []] | ]eqn:Htag; last done.
+    apply Htag_interp in Htag as (? & ? & _). lia.
+  }
+  iMod "Hnt" as "[Hnt Htag_auth]". iModIntro.
+  iSplitL "Hnt Hrel".
+  { destruct (decide (ot = nt)) as [-> | Hneq]. { iSplit; done. }
+    destruct nt. {  iSplit; first done. iRight. iExists t, t. eauto. }
+    iSplit; first done. by iLeft.
+  }
+
+  iAssert (⌜retag σ_t.(sst) σ_t.(snp) σ_t.(scs) c l ot rkind kind T = Some (nt, α', nxtp')⌝)%I as "%Hretag_t".
+  { iPoseProof (state_rel_calls_eq with "Hsrel") as "<-".
+    iPoseProof (state_rel_stacks_eq with "Hsrel") as "<-".
+    iPoseProof (state_rel_snp_eq with "Hsrel") as "<-". done. }
+
+  (* re-establishing the interpretation *)
+  iPoseProof (state_rel_get_pure with "Hsrel") as "%Hp".
+  iExists M_call, M_tag', M_t, M_s.
+  iFrame. iSplitL.
+  { (* state relation *)
+    rewrite /state_rel. simpl. iDestruct "Hsrel" as "(-> & %Hs_eq & %Hsnp_eq & -> & -> & Hsrel)".
+    do 5 (iSplitL; first done). iIntros (l' Hsl').
+    iDestruct ("Hsrel" $! l' with "[//]") as "[Hpub | [%t' %Hpriv]]"; first (iLeft; iApply "Hpub").
+    iRight. iPureIntro. exists t'.
+    (* private locations are preserved: t' cannot be part of the range affected by the retag, because that is public *)
+    destruct Hpriv as (tk' & Hsome_tk' & Ht_l' & Htk'). exists tk'.
+    split_and!; [ | done | done].
+    subst M_tag'. destruct (decide (ot = nt)) as [ | Hneq]; first done.
+    destruct nt as [ nt | ]; last done.
+    destruct (decide (t' = nt)) as [-> | Hneq']; first last.
+    { rewrite lookup_insert_ne; done. }
+    exfalso. (* contradiction with Hsome_tk' *)
+    destruct Hnt as [<- | [-> ->]]; first congruence.
+    apply Htag_interp in Hsome_tk' as (? & _). lia.
+  }
+  iSplitL.
+  { (* call interpretation. *)
+    iPureIntro. intros c' M' [Hc' HM']%Hcall_interp. simpl. split; first done.
+    specialize (retag_change_nxtp _ _ _ _ _ _ _ _ _ _ _ _ Hretag) as Hnxtp'.
+    intros t' S HS. simpl. specialize (HM' t' S HS) as (Ht' & Hprot).
+    split; first lia. intros l' Hl'.
+    specialize (Hprot l' Hl') as (s & pm' & Hs & Hit & Hpm').
+    specialize (retag_item_active_preserving _ _ _ _ _ _ _ _ _ _ _ _ Hretag_t l' s (Tagged t') c' pm' Hs Hc' Hit) as (s' & -> & Hin'). eauto.
+  }
+  iSplitL.
+  { (* tag interpretation. *)
+    destruct Htag_interp as (Htag_interp & Ht_dom & Hs_dom).
+    destruct Hp as (Hsst & Hsnp & Hsnc & Hscs).
+    iPureIntro. split_and!.
+    { intros t tk' Hsome.
+      assert ((nt = Tagged σ_t.(snp) ∧ t = σ_t.(snp) ∧ tk' = tk_pub ∧ nxtp' = S σ_t.(snp)) ∨ M_tag !! t = Some (tk', ())) as [(-> & -> & -> & ->) | Hsome'].
+      { subst M_tag'. destruct (decide (ot = nt)) as [<- | Hneq]; first by eauto.
+        destruct nt as [ nt | ]; last by eauto.
+        destruct Hnt as [<- | [-> ?]]; first congruence.
+        destruct (decide (t = σ_s.(snp))) as [-> | Hneq'].
+        - rewrite lookup_insert in Hsome. injection Hsome as [= <-]. left; naive_solver.
+        - rewrite lookup_insert_ne in Hsome; last done. by right.
+      }
+      - (* the new tag: nothing to show, since we don't put the tagged locations under control *)
+        simpl. set (nt := σ_t.(snp)).
+        assert (∀ l', M_t !! (nt, l') = None) as Mt_nt.
+        { intros l'. destruct (M_t !! (nt, l')) eqn:Heq; last done.
+          specialize (Ht_dom σ_t.(snp) l' ltac:(eauto)) as ([? []] & [? _]%Htag_interp). lia. }
+        assert (∀ l', M_s !! (nt, l') = None) as Ms_nt.
+        { intros l'. destruct (M_s !! (nt, l')) eqn:Heq; last done.
+          specialize (Hs_dom σ_t.(snp) l' ltac:(eauto)) as ([? []] & [? _]%Htag_interp). lia. }
+        split_and!; [lia | lia | | | ].
+        + intros l' sc_t HM_t. congruence.
+        + intros l' sc_s HM_s. congruence.
+        + apply dom_agree_on_tag_not_elem; done.
+      - (* old tags are preserved *)
+        simpl. specialize (Htag_interp _ _ Hsome') as (? & ? & Hcontrolled_t & Hcontrolled_s & Hdom).
+        split_and!; [lia | lia | | | ].
+        + intros. eapply retag_loc_controlled_preserved; [ done | done | | done | by apply Hcontrolled_t].
+          intros <-. move : Hpub. rewrite /untagged_or_public. congruence.
+        + intros. eapply retag_loc_controlled_preserved; [ done | done | | done | by apply Hcontrolled_s].
+          intros <-. move : Hpub. rewrite /untagged_or_public. congruence.
+        + done.
+    }
+    { subst M_tag'. destruct (decide (ot = nt)); first done. destruct nt as [nt | ]; last done.
+      intros. rewrite lookup_insert_is_Some'. right; eauto.
+    }
+    { subst M_tag'. destruct (decide (ot = nt)); first done. destruct nt as [nt | ]; last done.
+      intros. rewrite lookup_insert_is_Some'. right; eauto.
+    }
+  }
+  iSplit; done.
+Qed.
+
+Lemma sim_retag_public l_t l_s ot os c kind T rkind π Φ :
+  value_rel [ScPtr l_t ot] [ScPtr l_s os] -∗
+  (∀ nt, value_rel [ScPtr l_t nt] [ScPtr l_s nt] -∗
+    #[ScPtr l_t nt] ⪯{π, Ω} #[ScPtr l_s nt] [{ Φ }]) -∗
+  Retag #[ScPtr l_t ot] #[ScCallId c] kind T rkind ⪯{π, Ω} Retag #[ScPtr l_s os] #[ScCallId c] kind T rkind [{ Φ }].
+Proof.
+  rewrite {1}/value_rel big_sepL2_singleton.
+  iIntros "#Hscrel Hsim".
+  iPoseProof (sc_rel_ptr_source with "Hscrel") as "[%Heq Hpub]". injection Heq as [= -> <-].
+  iApply sim_lift_head_step_both. iIntros (??????) "((HP_t & HP_s & Hbor) & %Hthread & %Hsafe)".
+  (* exploit source to gain knowledge about stacks & that c is a valid id *)
+  specialize (pool_safe_irred _ _ _ _ _ _ _ Hsafe Hthread ltac:(done)) as (c' & ot' & l' & [= <- <-] & [= <-] & Hc_active & Hretag_some_s).
+  iPoseProof (bor_interp_get_pure with "Hbor") as "%Hp".
+  have Hretag_some_t : is_Some (retag σ_t.(sst) σ_t.(snp) σ_t.(scs) c l_s ot rkind kind T).
+  { destruct Hp as (<- & <- & _ & <- & _). done. }
+  iModIntro. iSplitR.
+  { iPureIntro.
+    destruct Hretag_some_t as ([[] ] & Hretag_some_t).
+    do 3 eexists. eapply retag_head_step'; last done.
+    destruct Hp as (_ & _ & _ & <- & _). done.
+  }
+  iIntros (e_t' efs_t σ_t') "%Hhead_t".
+  specialize (head_retag_inv _ _ _ _ _ _ _ _ _ _ _ Hhead_t) as (nt & α' & nxtp' & Hretag_t & -> & -> & -> & Hc).
+  have Hretag_s : retag σ_s.(sst) σ_s.(snp) σ_s.(scs) c l_s ot rkind kind T = Some (nt, α', nxtp').
+  { destruct Hp as (-> & -> & _ & -> & _). done. }
+  assert (Hhead_s : head_step P_s (Retag #[ScPtr l_s ot] #[ScCallId c] kind T rkind) σ_s #[ScPtr l_s nt]%E (mkState (shp σ_s) α' (scs σ_s) nxtp' (snc σ_s)) []).
+  { eapply retag_head_step'; done. }
+
+  iPoseProof (bor_interp_get_state_wf with "Hbor") as "[%Hwf_t %Hwf_s]".
+  iMod (bor_interp_retag_public _ _ _ _ _ _ _ _ _ _ _ Hretag_s with "Hscrel Hbor") as "[Hscrel' Hbor]".
+  { by eapply head_step_wf. }
+  { by eapply head_step_wf. }
+  iModIntro.
+
+  iExists #[ScPtr l_s nt]%E, [], (mkState σ_s.(shp) α' σ_s.(scs) nxtp' σ_s.(snc)).
+  iSplitR; first done.
+  iFrame "Hbor HP_t HP_s".
+  iSplitL; last done. iApply "Hsim". iApply big_sepL2_singleton. done.
+Qed.
+
+(** InitCall *)
+Lemma bor_interp_init_call σ_t σ_s :
+  bor_interp sc_rel σ_t σ_s ==∗
+  σ_t.(snc) @@ ∅ ∗
+  bor_interp sc_rel
+    (mkState σ_t.(shp) σ_t.(sst) ({[ σ_t.(snc) ]} ∪ σ_t.(scs)) σ_t.(snp) (S σ_t.(snc)))
+    (mkState σ_s.(shp) σ_s.(sst) ({[ σ_s.(snc) ]} ∪ σ_s.(scs)) σ_s.(snp) (S σ_s.(snc))).
+Proof.
+  iIntros "(% & % & % & % & (Hc & Htag_auth & Htag_t_auth & Htag_s_auth) & #Hsrel & %Hcall_interp & %Htag_interp & %Hwf_s & %Hwf_t)".
+  iPoseProof (state_rel_snc_eq with "Hsrel") as "%Hsnc_eq".
+  assert (M_call !! σ_t.(snc) = None) as Hfresh.
+  { destruct (M_call !! σ_t.(snc)) as [ M' | ] eqn:HM'; last done. apply Hcall_interp in HM' as (Hin & _).
+    apply Hwf_t in Hin. lia. }
+  iMod (ghost_map_insert σ_t.(snc) ∅ Hfresh with "Hc") as "[Hc Hcall]".
+  iModIntro. iFrame "Hcall".
+  iExists (<[σ_t.(snc) := ∅]> M_call), M_tag, M_t, M_s. iFrame.
+  iSplitL.
+  { iDestruct "Hsrel" as "(H1 & H2 & H3 & H4 & %H5 & H6)". rewrite /state_rel. simpl.
+    iFrame "H1 H2 H3".
+    iSplitR. { iPureIntro. lia. }
+    iSplitR. { rewrite H5 Hsnc_eq. done. }
+    iIntros (l Hl). iDestruct ("H6" $! l with "[//]") as "[Hpub | (%t & %Hpriv)]".
+    - iLeft. iApply "Hpub".
+    - iRight. iPureIntro. exists t.
+      destruct Hpriv as (tk & Htk & Hs & [-> | [-> (c' & Hin)]]).
+      { exists tk_local. split_and!; eauto. }
+      exists tk_unq. split_and!; [done.. | ]. right. split; first done.
+      exists c'. destruct Hin as (M' & HM' & Hin). exists M'.
+      split; last done. apply lookup_insert_Some. right. split; last done.
+      apply Hcall_interp in HM' as (Hwf_tag & _).
+      specialize (state_wf_cid_agree _ Hwf_t _ Hwf_tag). lia.
+  }
+  iSplitL.
+  { iPureIntro. intros c M'. simpl. rewrite lookup_insert_Some. intros [(<- & <-) | [Hneq Hsome]].
+    - split; first set_solver. intros ? ?. rewrite lookup_empty. congruence.
+    - rewrite elem_of_union. apply Hcall_interp in Hsome as [Hin Ha]. split; [by eauto | done].
+  }
+  iSplitL. { iPureIntro. apply Htag_interp. }
+  iSplitL. { iPureIntro. destruct Hwf_s. constructor; simpl; try done.
+    - intros l stk Hstk. apply state_wf_stack_item in Hstk.
+      destruct Hstk as [Hstk ?]. split; last done. intros i Hi. specialize (Hstk i Hi).
+      destruct tg, protector; naive_solver.
+    - intros c. rewrite elem_of_union elem_of_singleton. intros [-> | Hin%state_wf_cid_agree]; lia.
+  }
+  (* TODO: duplicated proof *)
+  iPureIntro. destruct Hwf_t. constructor; simpl; try done.
+  - intros l stk Hstk. apply state_wf_stack_item in Hstk.
+    destruct Hstk as [Hstk ?]. split; last done. intros i Hi. specialize (Hstk i Hi).
+    destruct tg, protector; naive_solver.
+  - intros c. rewrite elem_of_union elem_of_singleton. intros [-> | Hin%state_wf_cid_agree]; lia.
+Qed.
+
+Lemma sim_init_call π Φ :
+  (∀ c, c @@ ∅ -∗
+    #[ScCallId c] ⪯{π, Ω} #[ScCallId c] [{ Φ }]) -∗
+  InitCall ⪯{π, Ω} InitCall [{ Φ }].
+Proof.
+  iIntros "Hsim". iApply sim_lift_head_step_both. iIntros (??????) "((HP_t & HP_s & Hbor) & _ & _)".
+  iPoseProof (bor_interp_get_pure with "Hbor") as "%Hp".
+  iMod (bor_interp_init_call with "Hbor") as "[Hc Hbor]". iModIntro.
+  iSplitR.
+  { iPureIntro. do 3 eexists. eapply init_call_head_step. }
+  iIntros (e_t' efs_t σ_t') "%Hhead".
+  specialize (head_init_call_inv _ _ _ _ _ Hhead) as (c & Heqc & -> & -> & ->).
+  iModIntro. iExists (#[ScCallId σ_s.(snc)])%E, [], (mkState σ_s.(shp) σ_s.(sst) ({[ σ_s.(snc) ]} ∪ σ_s.(scs)) σ_s.(snp) (S σ_s.(snc))).
+  iSplitR. { iPureIntro. eapply init_call_head_step. }
+  iSplitR "Hsim Hc"; first last.
+  { iSplitL; last done. destruct Hp as (_ & _ & Heqc' & _). rewrite Heqc Heqc'. by iApply "Hsim". }
+  iFrame.
+Qed.
+
+
+(** EndCall *)
+Lemma bor_interp_end_call c σ_t σ_s :
+  bor_interp sc_rel σ_t σ_s -∗
+  c @@ ∅ ==∗ (* we need it to be empty to avoid tripping private locations *)
+  ⌜c ∈ σ_t.(scs) ∧ c ∈ σ_s.(scs)⌝ ∗ bor_interp sc_rel (state_upd_calls (.∖ {[ c ]}) σ_t) (state_upd_calls (.∖ {[ c ]}) σ_s).
+Proof.
+  iIntros "(% & % & % & % & (Hc & Htag_auth & Htag_t_auth & Htag_s_auth) & #Hsrel & %Hcall_interp & %Htag_interp & %Hwf_s & %Hwf_t) Hcall".
+  iPoseProof (ghost_map_lookup with "Hc Hcall") as "%Hlookup".
+  iMod (ghost_map_delete with "Hc Hcall") as "Hc". iModIntro.
+  iPoseProof (state_rel_calls_eq with "Hsrel") as "->".
+  iSplitR.
+  { destruct (Hcall_interp _ _ Hlookup) as (? & _). done. }
+  iExists (delete c M_call), M_tag, M_t, M_s. iFrame.
+  iSplitL "Hsrel".
+  { iDestruct "Hsrel" as "(H1 & H2 & H3 & H4 & %H5 & H6)". rewrite /state_rel. cbn.
+    iFrame "H1 H2 H3 H4".
+    iSplitR. { rewrite H5. done. }
+    iIntros (l Hl). iDestruct ("H6" $! l with "[//]") as "[Hpub | (%t & %Hpriv)]".
+    - iLeft. iApply "Hpub".
+    - iRight. iPureIntro. exists t.
+      destruct Hpriv as (tk & Htk & Hs & [-> | [-> (c' & Hin)]]).
+      { exists tk_local. split_and!; eauto. }
+      exists tk_unq. split_and!; [done.. | ]. right. split; first done.
+      exists c'. destruct Hin as (M' & HM' & Hin). exists M'.
+      assert (c ≠ c') as Hneq.
+      { intros <-. simplify_eq. destruct Hin as (L & Hsome & _).
+        rewrite lookup_empty in Hsome. done.
+      }
+      rewrite lookup_delete_ne; last done. done.
+  }
+  iSplitL.
+  { iPureIntro. by apply call_set_interp_remove. }
+  iSplitL.
+  { iPureIntro. apply Htag_interp. }
+  iSplitL.
+  { iPureIntro. destruct Hwf_s. constructor; [done.. | ].
+    intros c'. cbn. rewrite elem_of_difference. intros [Hin _]. eauto. }
+  iPureIntro. destruct Hwf_t. constructor; [done.. | ].
+  intros c'. cbn. rewrite elem_of_difference. intros [Hin _]. eauto.
+Qed.
+
+Lemma sim_endcall c π Φ :
+  c @@ ∅ -∗ (* needs to be empty so we don't trip private locations *)
+  #[☠] ⪯{π, Ω} #[☠] [{ Φ }] -∗
+  EndCall #[ScCallId c] ⪯{π, Ω} EndCall #[ScCallId c] [{ Φ }].
+Proof.
+  iIntros "Hcall Hsim". iApply sim_lift_head_step_both. iIntros (??????) "((HP_t & HP_s & Hbor) & _ & _)".
+  iMod (bor_interp_end_call with "Hbor Hcall") as "[%Hc_in Hbor]". iModIntro.
+  iSplitR.
+  { iPureIntro. do 3 eexists. eapply end_call_head_step. apply Hc_in. }
+  iIntros (e_t' efs_t σ_t') "%Hhead".
+  specialize (head_end_call_inv _ _ _ _ _ _ Hhead) as (_ & -> & -> & ->).
+  iModIntro. iExists (#[☠])%E, [], (state_upd_calls (.∖ {[ c ]}) σ_s).
+  iSplitR. { iPureIntro. eapply end_call_head_step. apply Hc_in. }
+  iSplitR "Hsim"; first last.
+  { iFrame "Hsim". done. }
+  iFrame.
+Qed.
+
+
+(** Call *)
+Lemma sim_call fn (r_t r_s : result) π Φ :
+  Ω r_t r_s -∗
+  (∀ r_t r_s : result, Ω r_t r_s -∗ Φ (of_result r_t) (of_result r_s)) -∗
+  Call #[ScFnPtr fn] r_t ⪯{π, Ω} Call #[ScFnPtr fn] r_s [{ Φ }].
+Proof.
+  iIntros "Hval Hsim". iApply (sim_lift_call _ _ _ fn r_t r_s with "Hval"). by iApply "Hsim".
+Qed.
+End lifting.
